instantiate muaux

thys/Monitor.thy
@@ -693,11 +693,23 @@ locale msaux =
   and valid_result_msaux: "valid_msaux w n L R aux auxlist \<Longrightarrow> result_msaux aux =
     foldr (\<union>) [rel. (t, rel) \<leftarrow> auxlist, left (ivl w) \<le> current w - t] {}"
 
+fun check_before :: "\<I> \<Rightarrow> ts \<Rightarrow> (ts \<times> 'a \<times> 'b) \<Rightarrow> bool" where
+  "check_before I dt (t, a, b) \<longleftrightarrow> enat t + right I < enat dt"
+
+fun proj_thd :: "('a \<times> 'b \<times> 'c) \<Rightarrow> 'c" where
+  "proj_thd (t, a1, a2) = a2"
+
 definition update_until :: "\<I> \<Rightarrow> bool \<Rightarrow> 'a table \<Rightarrow> 'a table \<Rightarrow> ts \<Rightarrow> 'a muaux \<Rightarrow> 'a muaux" where
   "update_until I pos rel1 rel2 nt aux =
     (map (\<lambda>x. case x of (t, a1, a2) \<Rightarrow> (t, if pos then join a1 True rel1 else a1 \<union> rel1,
       if mem (nt - t) I then a2 \<union> join rel2 pos a1 else a2)) aux) @
     [(nt, rel1, if left I = 0 then rel2 else empty_table)]"
+
+lemma map_proj_thd_update_until: "map proj_thd (takeWhile (check_before I nt) auxlist) =
+  map proj_thd (takeWhile (check_before I nt) (update_until I pos rel1 rel2 nt auxlist))"
+  apply (induction auxlist)
+   apply (auto simp add: update_until_def split: if_splits)
+  by (smt ab_semigroup_add_class.add_ac(1) leD le_cases le_iff_add ordered_cancel_comm_monoid_diff_class.add_diff_inverse plus_enat_simps(1))+
 
 fun eval_until :: "\<I> \<Rightarrow> ts \<Rightarrow> 'a muaux \<Rightarrow> 'a table list \<times> 'a muaux" where
   "eval_until I nt [] = ([], [])"
@@ -709,21 +721,31 @@ lemma eval_until_length:
   by (induction I nt auxlist arbitrary: res auxlist' rule: eval_until.induct)
      (auto split: if_splits prod.splits)
 
+lemma eval_until_res: "eval_until I nt auxlist = (res, auxlist') \<Longrightarrow>
+  res = map proj_thd (takeWhile (check_before I nt) auxlist)"
+  by (induction I nt auxlist arbitrary: res auxlist' rule: eval_until.induct)
+     (auto split: prod.splits)
+
+lemma eval_until_auxlist': "eval_until I nt auxlist = (res, auxlist') \<Longrightarrow>
+  auxlist' = drop (length res) auxlist"
+  by (induction I nt auxlist arbitrary: res auxlist' rule: eval_until.induct)
+     (auto split: if_splits prod.splits)
+
 locale muaux =
-  fixes valid_muaux :: "window \<Rightarrow> nat \<Rightarrow> nat set \<Rightarrow> nat set \<Rightarrow> 'muaux \<Rightarrow> 'a muaux \<Rightarrow> bool"
-  and init_muaux :: "\<I> \<Rightarrow> nat \<Rightarrow> nat set \<Rightarrow> nat set \<Rightarrow> 'muaux"
-  and add_new_muaux :: "bool \<Rightarrow> 'a table \<Rightarrow> 'a table \<Rightarrow> ts \<Rightarrow> 'muaux \<Rightarrow> 'muaux"
+  fixes valid_muaux :: "window \<Rightarrow> bool \<Rightarrow> nat \<Rightarrow> nat set \<Rightarrow> nat set \<Rightarrow> 'muaux \<Rightarrow> 'a muaux \<Rightarrow> bool"
+  and init_muaux :: "\<I> \<Rightarrow> bool \<Rightarrow> nat \<Rightarrow> nat set \<Rightarrow> nat set \<Rightarrow> 'muaux"
+  and add_new_muaux :: "'a table \<Rightarrow> 'a table \<Rightarrow> ts \<Rightarrow> 'muaux \<Rightarrow> 'muaux"
   and length_muaux :: "'muaux \<Rightarrow> nat"
   and eval_muaux :: "nat \<Rightarrow> 'muaux \<Rightarrow> 'a table list \<times> 'muaux"
-  assumes valid_init_muaux: "L \<subseteq> R \<Longrightarrow> valid_muaux (init_window I) n L R (init_muaux I n L R) []"
-  assumes valid_add_new_muaux: "valid_muaux w n L R aux auxlist \<Longrightarrow> table n L rel1 \<Longrightarrow> table n R rel2 \<Longrightarrow>
+  assumes valid_init_muaux: "L \<subseteq> R \<Longrightarrow> valid_muaux (init_window I) pos n L R (init_muaux I pos n L R) []"
+  assumes valid_add_new_muaux: "valid_muaux w pos n L R aux auxlist \<Longrightarrow> table n L rel1 \<Longrightarrow> table n R rel2 \<Longrightarrow>
     nt \<ge> current w \<Longrightarrow> w' = w\<lparr>current := nt\<rparr> \<Longrightarrow>
-    valid_muaux w' n L R (add_new_muaux pos rel1 rel2 nt aux)
+    valid_muaux w' pos n L R (add_new_muaux rel1 rel2 nt aux)
     (update_until (ivl w) pos rel1 rel2 nt auxlist)"
-  assumes valid_length_muaux: "valid_muaux w n L R aux auxlist \<Longrightarrow> length_muaux aux = length auxlist"
-  assumes valid_eval_muaux: "valid_muaux w n L R aux auxlist \<Longrightarrow> nt \<ge> current w \<Longrightarrow>
+  assumes valid_length_muaux: "valid_muaux w pos n L R aux auxlist \<Longrightarrow> length_muaux aux = length auxlist"
+  assumes valid_eval_muaux: "valid_muaux w pos n L R aux auxlist \<Longrightarrow> nt \<ge> current w \<Longrightarrow>
     eval_muaux nt aux = (res, aux') \<Longrightarrow> eval_until (ivl w) nt auxlist = (res', auxlist') \<Longrightarrow>
-    res = res' \<and> valid_muaux w n L R aux' auxlist'"
+    res = res' \<and> valid_muaux w pos n L R aux' auxlist'"
 
 locale maux = msaux valid_msaux init_msaux filter_msaux join_msaux add_new_msaux result_msaux +
   muaux valid_muaux init_muaux add_new_muaux length_muaux eval_muaux
@@ -733,9 +755,9 @@ locale maux = msaux valid_msaux init_msaux filter_msaux join_msaux add_new_msaux
   and join_msaux :: "bool \<Rightarrow> 'a table \<Rightarrow> 'msaux \<Rightarrow> 'msaux"
   and add_new_msaux :: "nat \<times> 'a table \<Rightarrow> 'msaux \<Rightarrow> 'msaux"
   and result_msaux :: "'msaux \<Rightarrow> 'a table"
-  and valid_muaux :: "window \<Rightarrow> nat \<Rightarrow> nat set \<Rightarrow> nat set \<Rightarrow> 'muaux \<Rightarrow> 'a muaux \<Rightarrow> bool"
-  and init_muaux :: "\<I> \<Rightarrow> nat \<Rightarrow> nat set \<Rightarrow> nat set \<Rightarrow> 'muaux"
-  and add_new_muaux :: "bool \<Rightarrow> 'a table \<Rightarrow> 'a table \<Rightarrow> ts \<Rightarrow> 'muaux \<Rightarrow> 'muaux"
+  and valid_muaux :: "window \<Rightarrow> bool \<Rightarrow> nat \<Rightarrow> nat set \<Rightarrow> nat set \<Rightarrow> 'muaux \<Rightarrow> 'a muaux \<Rightarrow> bool"
+  and init_muaux :: "\<I> \<Rightarrow> bool \<Rightarrow> nat \<Rightarrow> nat set \<Rightarrow> nat set \<Rightarrow> 'muaux"
+  and add_new_muaux :: "'a table \<Rightarrow> 'a table \<Rightarrow> ts \<Rightarrow> 'muaux \<Rightarrow> 'muaux"
   and length_muaux :: "'muaux \<Rightarrow> nat"
   and eval_muaux :: "nat \<Rightarrow> 'muaux \<Rightarrow> 'a table list \<times> 'muaux"
 
@@ -765,9 +787,9 @@ function (in maux) (sequential) minit0 :: "nat \<Rightarrow> 'a Formula.formula 
       Formula.Neg \<phi> \<Rightarrow> MSince False (minit0 n \<phi>) I (minit0 n \<psi>) ([], []) [] (init_msaux I n (Formula.fv \<phi>) (Formula.fv \<psi>))
     | _ \<Rightarrow> undefined))"
 | "minit0 n (Formula.Until \<phi> I \<psi>) = (if safe_formula \<phi>
-    then MUntil True (minit0 n \<phi>) I (minit0 n \<psi>) ([], []) [] (init_muaux I n (Formula.fv \<phi>) (Formula.fv \<psi>))
+    then MUntil True (minit0 n \<phi>) I (minit0 n \<psi>) ([], []) [] (init_muaux I True n (Formula.fv \<phi>) (Formula.fv \<psi>))
     else (case \<phi> of
-      Formula.Neg \<phi> \<Rightarrow> MUntil False (minit0 n \<phi>) I (minit0 n \<psi>) ([], []) [] (init_muaux I n (Formula.fv \<phi>) (Formula.fv \<psi>))
+      Formula.Neg \<phi> \<Rightarrow> MUntil False (minit0 n \<phi>) I (minit0 n \<psi>) ([], []) [] (init_muaux I False n (Formula.fv \<phi>) (Formula.fv \<psi>))
     | _ \<Rightarrow> undefined))"
 | "minit0 n (Formula.MatchP I r) =
     (let (mr, \<phi>s) = to_mregex r
@@ -979,7 +1001,7 @@ primrec (in maux) meval :: "nat \<Rightarrow> ts \<Rightarrow> 'a Formula.databa
     in (zs, MSince pos \<phi> I \<psi> buf nts aux))"
 | "meval n t db (MUntil pos \<phi> I \<psi> buf nts aux) =
     (let (xs, \<phi>) = meval n t db \<phi>; (ys, \<psi>) = meval n t db \<psi>;
-      (aux, buf, nts) = mbuf2t_take (add_new_muaux pos) aux (mbuf2_add xs ys buf) (nts @ [t]);
+      (aux, buf, nts) = mbuf2t_take add_new_muaux aux (mbuf2_add xs ys buf) (nts @ [t]);
       (zs, aux) = eval_muaux (case nts of [] \<Rightarrow> t | nt # _ \<Rightarrow> nt) aux
     in (zs, MUntil pos \<phi> I \<psi> buf nts aux))"
 | "meval n t db (MMatchP I mr mrs \<phi>s buf nts aux) =
@@ -1597,14 +1619,14 @@ definition wf_until_auxlist :: "'a Formula.trace \<Rightarrow> nat \<Rightarrow>
 definition (in muaux) wf_until_aux :: "'a Formula.trace \<Rightarrow> nat \<Rightarrow> 'a list set \<Rightarrow> bool \<Rightarrow>
     'a Formula.formula \<Rightarrow> \<I> \<Rightarrow> 'a Formula.formula \<Rightarrow> 'muaux \<Rightarrow> nat \<Rightarrow> bool" where
   "wf_until_aux \<sigma> n R pos \<phi> I \<psi> aux ne \<longleftrightarrow> Formula.fv \<phi> \<subseteq> Formula.fv \<psi> \<and>
-    (\<exists>auxlist w. valid_muaux w n (Formula.fv \<phi>) (Formula.fv \<psi>) aux auxlist \<and>
+    (\<exists>auxlist w. valid_muaux w pos n (Formula.fv \<phi>) (Formula.fv \<psi>) aux auxlist \<and>
       ivl w = I \<and>
       current w = (if ne + length auxlist = 0 then 0 else \<tau> \<sigma> (ne + length auxlist - 1)) \<and>
       wf_until_auxlist \<sigma> n R pos \<phi> I \<psi> auxlist ne)"
 
 lemma (in muaux) wf_until_aux_UNIV_alt:
   "wf_until_aux \<sigma> n UNIV pos \<phi> I \<psi> aux ne \<longleftrightarrow> Formula.fv \<phi> \<subseteq> Formula.fv \<psi> \<and>
-    (\<exists>auxlist w. valid_muaux w n (Formula.fv \<phi>) (Formula.fv \<psi>) aux auxlist \<and>
+    (\<exists>auxlist w. valid_muaux w pos n (Formula.fv \<phi>) (Formula.fv \<psi>) aux auxlist \<and>
       ivl w = I \<and>
       current w = (if ne + length auxlist = 0 then 0 else \<tau> \<sigma> (ne + length auxlist - 1)) \<and>
       list_all2 (\<lambda>x i. case x of (t, r1, r2) \<Rightarrow> t = \<tau> \<sigma> i \<and>
@@ -1755,7 +1777,7 @@ lemma wf_ts_regex_0: "wf_ts_regex \<sigma> 0 r []"
 lemma (in msaux) wf_since_aux_Nil: "Formula.fv \<phi>' \<subseteq> Formula.fv \<psi>' \<Longrightarrow> wf_since_aux \<sigma> n R pos \<phi>' I \<psi>' (init_msaux I n (Formula.fv \<phi>') (Formula.fv \<psi>')) 0"
   unfolding wf_since_aux_def by (auto simp: init_window_def intro!: exI[of _ "[]"] exI[of _ "init_window I"] valid_init_msaux)
 
-lemma (in muaux) wf_until_aux_Nil: "Formula.fv \<phi>' \<subseteq> Formula.fv \<psi>' \<Longrightarrow> wf_until_aux \<sigma> n R pos \<phi>' I \<psi>' (init_muaux I n (Formula.fv \<phi>') (Formula.fv \<psi>')) 0"
+lemma (in muaux) wf_until_aux_Nil: "Formula.fv \<phi>' \<subseteq> Formula.fv \<psi>' \<Longrightarrow> wf_until_aux \<sigma> n R pos \<phi>' I \<psi>' (init_muaux I pos n (Formula.fv \<phi>') (Formula.fv \<psi>')) 0"
   unfolding wf_until_aux_def wf_until_auxlist_def by (auto simp: init_window_def intro!: exI[of _ "[]"] exI[of _ "init_window I"] valid_init_muaux)
 
 lemma wf_matchP_aux_Nil: "wf_matchP_aux \<sigma> n R I r [] 0"
@@ -3198,10 +3220,10 @@ lemma (in muaux) wf_update_until:
       and qtable1: "qtable n (Formula.fv \<phi>) (mem_restr R) (\<lambda>v. Formula.sat \<sigma> (map the v) (ne + length_muaux aux) \<phi>) rel1"
       and qtable2: "qtable n (Formula.fv \<psi>) (mem_restr R) (\<lambda>v. Formula.sat \<sigma> (map the v) (ne + length_muaux aux) \<psi>) rel2"
       and fvi_subset: "Formula.fv \<phi> \<subseteq> Formula.fv \<psi>"
-    shows "wf_until_aux \<sigma> n R pos \<phi> I \<psi> (add_new_muaux pos rel1 rel2 (\<tau> \<sigma> (ne + length_muaux aux)) aux) ne \<and>
-      length_muaux (add_new_muaux pos rel1 rel2 (\<tau> \<sigma> (ne + length_muaux aux)) aux) = Suc (length_muaux aux)"
+    shows "wf_until_aux \<sigma> n R pos \<phi> I \<psi> (add_new_muaux rel1 rel2 (\<tau> \<sigma> (ne + length_muaux aux)) aux) ne \<and>
+      length_muaux (add_new_muaux rel1 rel2 (\<tau> \<sigma> (ne + length_muaux aux)) aux) = Suc (length_muaux aux)"
 proof -
-  from pre obtain auxlist w where valid_aux: "valid_muaux w n (Formula.fv \<phi>) (Formula.fv \<psi>) aux auxlist" and
+  from pre obtain auxlist w where valid_aux: "valid_muaux w pos n (Formula.fv \<phi>) (Formula.fv \<psi>) aux auxlist" and
     ivl_w: "ivl w = I" and current_w: "current w = (if ne + length auxlist = 0 then 0 else \<tau> \<sigma> (ne + length auxlist - 1))" and
     pre_list: "wf_until_auxlist \<sigma> n R pos \<phi> I \<psi> auxlist ne"
     unfolding wf_until_aux_def by auto
@@ -3219,10 +3241,10 @@ proof -
     using qtable2 by (auto simp add: qtable_def)
   have fv_sub: "fv \<phi> \<subseteq> fv \<psi>"
     using pre unfolding wf_until_aux_def by auto
-  moreover have valid_add_new_auxlist: "valid_muaux (w\<lparr>current := nt\<rparr>) n (fv \<phi>) (fv \<psi>) (add_new_muaux pos rel1 rel2 nt aux) auxlist'"
+  moreover have valid_add_new_auxlist: "valid_muaux (w\<lparr>current := nt\<rparr>) pos n (fv \<phi>) (fv \<psi>) (add_new_muaux rel1 rel2 nt aux) auxlist'"
     using valid_add_new_muaux[OF valid_aux tab1 tab2 nt_mono refl]
     unfolding auxlist'_def nt_def length_aux ivl_w .
-  moreover have "length_muaux (add_new_muaux pos rel1 rel2 nt aux) = Suc (length_muaux aux)"
+  moreover have "length_muaux (add_new_muaux rel1 rel2 nt aux) = Suc (length_muaux aux)"
     using valid_length_muaux[OF valid_add_new_auxlist] unfolding length_auxlist' length_aux[symmetric] .
   moreover have "wf_until_auxlist \<sigma> n R pos \<phi> I \<psi> auxlist' ne"
     using wf_update_until_auxlist[OF pre_list qtable1[unfolded length_aux] qtable2[unfolded length_aux] fv_sub]
@@ -4219,7 +4241,7 @@ next
     fix xs ys zs aux' aux'' buf' nts'
     assume eval_\<phi>: "fst (meval n (\<tau> \<sigma> j) (\<Gamma> \<sigma> j) \<phi>) = xs"
       and eval_\<psi>: "fst (meval n (\<tau> \<sigma> j) (\<Gamma> \<sigma> j) \<psi>) = ys"
-      and eq1: "mbuf2t_take (add_new_muaux pos) aux (mbuf2_add xs ys buf) (nts @ [\<tau> \<sigma> j]) =
+      and eq1: "mbuf2t_take add_new_muaux aux (mbuf2_add xs ys buf) (nts @ [\<tau> \<sigma> j]) =
         (aux', buf', nts')"
       and eq2: "eval_muaux (case nts' of [] \<Rightarrow> \<tau> \<sigma> j | nt # _ \<Rightarrow> nt) aux' = (zs, aux'')"
     define ne where "ne \<equiv> progress \<sigma> (Formula.Until \<phi>''' I \<psi>'') j"
@@ -4229,7 +4251,7 @@ next
         eval_\<psi> nts_snoc nts_snoc length_aux aux fvi_subset
       unfolding \<phi>'''
       by (elim mbuf2t_take_add_induct'[where j'="Suc j", OF eq1 buf]) (auto simp: ne_def wf_update_until)
-    then obtain auxlist' w where valid_aux': "valid_muaux w n (Formula.fv \<phi>'') (Formula.fv \<psi>'') aux' auxlist'" and
+    then obtain auxlist' w where valid_aux': "valid_muaux w pos n (Formula.fv \<phi>'') (Formula.fv \<psi>'') aux' auxlist'" and
       ivl_w: "ivl w = I" and current_w: "current w = (if ne + length auxlist' = 0 then 0 else \<tau> \<sigma> (ne + length auxlist' - 1))" and
       wf_auxlist': "wf_until_auxlist \<sigma> n R pos \<phi>'' I \<psi>'' auxlist' (progress \<sigma> (Formula.Until \<phi>''' I \<psi>'') j)"
       unfolding wf_until_aux_def ne_def by auto
@@ -4263,7 +4285,7 @@ next
         apply (auto split: if_splits list.splits)
         using \<tau>_mono diff_le_self by blast
     qed
-    have valid_aux'': "valid_muaux w n (fv \<phi>'') (fv \<psi>'') aux'' auxlist''"
+    have valid_aux'': "valid_muaux w pos n (fv \<phi>'') (fv \<psi>'') aux'' auxlist''"
       using valid_eval_muaux[OF valid_aux' current_w_le eq2, of zs'' auxlist'']
       by (auto simp add: zs''_def auxlist''_def)
     have length_aux'': "length_muaux aux'' = length auxlist''"
