thys/Optimized_MTL.thy
@@ -7,61 +7,131 @@ begin
 lemma less_enat_iff: "a < enat i \<longleftrightarrow> (\<exists>j. a = enat j \<and> j < i)"
   by (cases a) auto
 
-(* Optimized since data structure *)
+(* Optimized queue data structure *)
 
-type_synonym 'a queue = "'a list \<times> 'a list"
+type_synonym 'a queue_t = "'a list \<times> 'a list"
 
-definition linearize :: "'a queue \<Rightarrow> 'a list" where
-  "linearize q = (case q of (ls, fs) \<Rightarrow> ls @ rev fs)"
+typedef 'a queue = "{q :: 'a queue_t. case q of ([], []) \<Rightarrow> True | (fs, l # ls) \<Rightarrow> True
+  | _ \<Rightarrow> False}"
+  by (auto split: list.splits)
 
-definition empty_queue :: "'a queue" where
-  "empty_queue = ([], [])"
+setup_lifting type_definition_queue
+
+lift_definition linearize :: "'a queue \<Rightarrow> 'a list" is "(\<lambda>q. case q of (fs, ls) \<Rightarrow> fs @ rev ls)" .
+
+lift_definition empty_queue :: "'a queue" is "([], [])"
+  by (auto split: list.splits)
 
 lemma empty_queue_rep: "linearize empty_queue = []"
-  unfolding empty_queue_def by (simp add: linearize_def)
+  by transfer (simp add: empty_queue_def linearize_def)
 
-definition prepend_queue :: "'a \<Rightarrow> 'a queue \<Rightarrow> 'a queue" where
-  "prepend_queue a q = (case q of (ls, fs) \<Rightarrow> (a # ls, fs))"
+lift_definition is_empty :: "'a queue \<Rightarrow> bool" is "\<lambda>q. (case q of ([], []) \<Rightarrow> True | _ \<Rightarrow> False)" .
+
+lemma linearize_t_Nil: "(case q of (fs, ls) \<Rightarrow> fs @ rev ls) = [] \<longleftrightarrow> q = ([], [])"
+  by (auto split: prod.splits)
+
+lemma is_empty_alt: "is_empty q \<longleftrightarrow> linearize q = []"
+  apply transfer
+  unfolding linearize_t_Nil
+  by (metis (no_types, lifting) case_prodE case_prod_unfold list.case_eq_if snd_conv)
+
+fun prepend_queue_t :: "'a \<Rightarrow> 'a queue_t \<Rightarrow> 'a queue_t" where
+  "prepend_queue_t a ([], []) = ([], [a])"
+| "prepend_queue_t a (fs, l # ls) = (a # fs, l # ls)"
+| "prepend_queue_t a (f # fs, []) = undefined"
+
+lift_definition prepend_queue :: "'a \<Rightarrow> 'a queue \<Rightarrow> 'a queue" is prepend_queue_t
+  by (auto split: list.splits elim: prepend_queue_t.elims)
 
 lemma prepend_queue_rep: "linearize (prepend_queue a q) = a # linearize q"
-  by (auto simp add: linearize_def prepend_queue_def split: prod.splits)
+  by transfer (auto simp add: linearize_def elim: prepend_queue_t.elims split: prod.splits)
 
-definition append_queue :: "'a \<Rightarrow> 'a queue \<Rightarrow> 'a queue" where
-  "append_queue a q = (case q of (ls, fs) \<Rightarrow> (ls, a # fs))"
+lift_definition append_queue :: "'a \<Rightarrow> 'a queue \<Rightarrow> 'a queue" is
+  "(\<lambda>a q. case q of (fs, ls) \<Rightarrow> (fs, a # ls))"
+  by (auto split: list.splits)
 
 lemma append_queue_rep: "linearize (append_queue a q) = linearize q @ [a]"
-  by (auto simp add: linearize_def append_queue_def split: prod.splits)
+  by transfer (auto simp add: linearize_def split: prod.splits)
 
-fun safe_hd :: "'a queue \<Rightarrow> 'a option \<times> 'a queue" where
-  "safe_hd ([], []) = (None, ([], []))"
-| "safe_hd ([], fs) = (let ls = rev fs in (Some (hd ls), (ls, [])))"
-| "safe_hd (a # as, fs) = (Some a, (a # as, fs))"
+fun safe_last_t :: "'a queue_t \<Rightarrow> 'a option \<times> 'a queue_t" where
+  "safe_last_t ([], []) = (None, ([], []))"
+| "safe_last_t (fs, l # ls) = (Some l, (fs, l # ls))"
+| "safe_last_t (f # fs, []) = undefined"
+
+lift_definition safe_last :: "'a queue \<Rightarrow> 'a option \<times> 'a queue" is safe_last_t
+  by (auto split: prod.splits list.splits)
+
+lemma safe_last_rep: "safe_last q = (\<alpha>, q') \<Longrightarrow> linearize q = linearize q' \<and>
+  (case \<alpha> of None \<Rightarrow> linearize q = [] | Some a \<Rightarrow> linearize q \<noteq> [] \<and> a = last (linearize q))"
+  by transfer (auto split: list.splits elim: safe_last_t.elims)
+
+fun safe_hd_t :: "'a queue_t \<Rightarrow> 'a option \<times> 'a queue_t" where
+  "safe_hd_t ([], []) = (None, ([], []))"
+| "safe_hd_t ([], [l]) = (Some l, ([], [l]))"
+| "safe_hd_t ([], l # ls) = (let fs = rev ls in (Some (hd fs), (fs, [l])))"
+| "safe_hd_t (f # fs, l # ls) = (Some f, (f # fs, l # ls))"
+| "safe_hd_t (f # fs, []) = undefined"
+
+lift_definition(code_dt) safe_hd :: "'a queue \<Rightarrow> 'a option \<times> 'a queue" is safe_hd_t
+  apply (auto split: prod.splits list.splits)
+  subgoal for l ls
+    by (cases ls) (auto simp add: Let_def)
+  done
 
 lemma safe_hd_rep: "safe_hd q = (\<alpha>, q') \<Longrightarrow> linearize q = linearize q' \<and>
   (case \<alpha> of None \<Rightarrow> linearize q = [] | Some a \<Rightarrow> linearize q \<noteq> [] \<and> a = hd (linearize q))"
-  by (auto simp add: linearize_def Let_def split: prod.splits option.splits elim: safe_hd.elims)
+  by transfer (auto simp add: Let_def hd_append split: list.splits elim: safe_hd_t.elims)
 
-lemma safe_hd_Cons: "xs \<noteq> [] \<Longrightarrow> safe_hd (xs, []) = (Some (hd xs), (xs, []))"
-  by (cases xs) auto
+fun replace_hd_t :: "'a \<Rightarrow> 'a queue_t \<Rightarrow> 'a queue_t" where
+  "replace_hd_t a ([], []) = ([], [])"
+| "replace_hd_t a ([], [l]) = ([], [a])"
+| "replace_hd_t a ([], l # ls) = (let fs = rev ls in (a # tl fs, [l]))"
+| "replace_hd_t a (f # fs, l # ls) = (a # fs, l # ls)"
+| "replace_hd_t a (f # fs, []) = undefined"
 
-lemma safe_hd_idem: "safe_hd q = (a, q') \<Longrightarrow> safe_hd q' = (a, q')"
-  by (auto simp add: Let_def safe_hd_Cons elim: safe_hd.elims)
+lift_definition replace_hd :: "'a \<Rightarrow> 'a queue \<Rightarrow> 'a queue" is replace_hd_t
+  by (auto split: list.splits elim: replace_hd_t.elims)
 
-fun tl_queue :: "'a queue \<Rightarrow> 'a queue" where
-  "tl_queue ([], fs) = (tl (rev fs), [])"
-| "tl_queue (a # as, fs) = (as, fs)"
+lemma replace_hd_rep: "linearize q = f # fs \<Longrightarrow> linearize (replace_hd a q) = a # fs"
+  apply transfer
+  apply (auto split: list.splits prod.splits elim!: replace_hd_t.elims)
+  by (metis butlast.simps(2) butlast_append last_ConsR last_appendR list.distinct(1) list.sel(3)
+      snoc_eq_iff_butlast)+
 
-lemma tl_queue_rep: "linearize (tl_queue q) = tl (linearize q)"
-  by (auto simp add: linearize_def split: prod.splits elim: tl_queue.elims)
+fun replace_last_t :: "'a \<Rightarrow> 'a queue_t \<Rightarrow> 'a queue_t" where
+  "replace_last_t a ([], []) = ([], [])"
+| "replace_last_t a (fs, l # ls) = (fs, a # ls)"
+| "replace_last_t a (fs, []) = undefined"
 
-lemma length_tl_queue_rep: "linearize q \<noteq> [] \<Longrightarrow>
+lift_definition replace_last :: "'a \<Rightarrow> 'a queue \<Rightarrow> 'a queue" is replace_last_t
+  by (auto split: list.splits elim: replace_last_t.elims)
+
+lemma replace_last_rep: "linearize q = fs @ [f] \<Longrightarrow> linearize (replace_last a q) = fs @ [a]"
+  by transfer (auto split: list.splits prod.splits elim!: replace_last_t.elims)
+
+fun tl_queue_t :: "'a queue_t \<Rightarrow> 'a queue_t" where
+  "tl_queue_t ([], []) = ([], [])"
+| "tl_queue_t ([], [l]) = ([], [])"
+| "tl_queue_t ([], l # ls) = (tl (rev ls), [l])"
+| "tl_queue_t (a # as, fs) = (as, fs)"
+
+lift_definition tl_queue :: "'a queue \<Rightarrow> 'a queue" is tl_queue_t
+  by (auto split: list.splits elim!: tl_queue_t.elims)
+
+lemma tl_queue_rep: "\<not>is_empty q \<Longrightarrow> linearize (tl_queue q) = tl (linearize q)"
+  apply transfer
+  apply (auto split: prod.splits list.splits elim!: tl_queue_t.elims)
+  by (metis append.assoc append_Cons append_Nil list.sel(3) tl_append2)
+
+lemma length_tl_queue_rep: "\<not>is_empty q \<Longrightarrow>
   length (linearize (tl_queue q)) < length (linearize q)"
-  unfolding tl_queue_rep by simp
+  by transfer (auto split: prod.splits list.splits elim: tl_queue_t.elims)
 
 lemma length_tl_queue_safe_hd:
   assumes "safe_hd q = (Some a, q')"
   shows "length (linearize (tl_queue q')) < length (linearize q)"
-  using safe_hd_rep[OF assms] by (auto simp add: length_tl_queue_rep)
+  using safe_hd_rep[OF assms]
+  by (auto simp add: length_tl_queue_rep is_empty_alt)
 
 function dropWhile_queue :: "('a \<Rightarrow> bool) \<Rightarrow> 'a queue \<Rightarrow> 'a queue" where
   "dropWhile_queue f q = (case safe_hd q of (None, q') \<Rightarrow> q'
@@ -77,7 +147,7 @@ lemma dropWhile_hd_tl: "xs \<noteq> [] \<Longrightarrow>
 
 lemma dropWhile_queue_rep: "linearize (dropWhile_queue f q) = dropWhile f (linearize q)"
   by (induction f q rule: dropWhile_queue.induct)
-     (auto simp add: safe_hd_idem tl_queue_rep dropWhile_hd_tl
+     (auto simp add: tl_queue_rep dropWhile_hd_tl is_empty_alt
       split: prod.splits option.splits dest: safe_hd_rep)
 
 function takeWhile_queue :: "('a \<Rightarrow> bool) \<Rightarrow> 'a queue \<Rightarrow> 'a queue" where
@@ -96,7 +166,7 @@ lemma takeWhile_hd_tl: "xs \<noteq> [] \<Longrightarrow>
 
 lemma takeWhile_queue_rep: "linearize (takeWhile_queue f q) = takeWhile f (linearize q)"
   by (induction f q rule: takeWhile_queue.induct)
-     (auto simp add: prepend_queue_rep tl_queue_rep empty_queue_rep takeWhile_hd_tl
+     (auto simp add: prepend_queue_rep tl_queue_rep empty_queue_rep takeWhile_hd_tl is_empty_alt
       split: prod.splits option.splits dest: safe_hd_rep)
 
 function takedropWhile_queue :: "('a \<Rightarrow> bool) \<Rightarrow> 'a queue \<Rightarrow> 'a queue \<times> 'a list" where
@@ -116,8 +186,10 @@ lemma takedropWhile_queue_fst: "fst (takedropWhile_queue f q) = dropWhile_queue 
 lemma takedropWhile_queue_snd: "snd (takedropWhile_queue f q) = takeWhile f (linearize q)"
   apply (induction f q rule: takedropWhile_queue.induct)
   by (auto split: prod.splits)
-     (auto simp add: case_prod_unfold tl_queue_rep takeWhile_hd_tl
+     (auto simp add: case_prod_unfold tl_queue_rep takeWhile_hd_tl is_empty_alt
       split: option.splits dest: safe_hd_rep)
+
+(* Optimized since data structure *)
 
 type_synonym 'a mmsaux = "ts \<times> ts \<times> \<I> \<times> bool list \<times> bool list \<times>
   (ts \<times> 'a table) queue \<times> (ts \<times> 'a table) queue \<times>
@@ -284,12 +356,21 @@ lemma dropWhile_filter':
   using iffD1[OF filter_id_conv[symmetric], symmetric, of _ "\<lambda>(t, X). nt - t < c"]
   dual_order.trans by auto fastforce
 
+lemma dropWhile_filter'':
+  "sorted xs \<Longrightarrow> \<forall>t \<in> set xs. t \<le> nt \<Longrightarrow>
+  dropWhile (\<lambda>t. enat (nt - t) > c) xs = filter (\<lambda>t. enat (nt - t) \<le> c) xs"
+  apply (induction xs)
+   apply auto
+  apply (rule iffD1[OF filter_id_conv[symmetric], symmetric, of _ "\<lambda>t. enat (nt - t) \<le> c"])
+  using dual_order.trans by fastforce
+
 lemma takeWhile_filter:
   "sorted (map fst xs) \<Longrightarrow> \<forall>t \<in> fst ` set xs. t \<le> nt \<Longrightarrow>
   takeWhile (\<lambda>(t, X). enat (nt - t) > c) xs = filter (\<lambda>(t, X). enat (nt - t) > c) xs"
   apply (induction xs)
-  using iffD1[OF filter_empty_conv[symmetric], symmetric, of _ "\<lambda>(t, X). enat (nt - t) > c"]
-  less_enat_iff by auto fastforce
+   apply auto
+  apply (rule iffD1[OF filter_empty_conv[symmetric], symmetric, of _ "\<lambda>(t, X). enat (nt - t) > c"])
+  by (auto simp add: less_enat_iff)
 
 lemma takeWhile_filter':
   fixes nt :: nat
@@ -298,6 +379,14 @@ lemma takeWhile_filter':
   apply (induction xs)
   using iffD1[OF filter_empty_conv[symmetric], symmetric, of _ "\<lambda>(t, X). nt - t \<ge> c"]
   less_enat_iff by auto fastforce
+
+lemma takeWhile_filter'':
+  "sorted xs \<Longrightarrow> \<forall>t \<in> set xs. t \<le> nt \<Longrightarrow>
+  takeWhile (\<lambda>t. enat (nt - t) > c) xs = filter (\<lambda>t. enat (nt - t) > c) xs"
+  apply (induction xs)
+   apply auto
+  apply (rule iffD1[OF filter_empty_conv[symmetric], symmetric, of _ "\<lambda>t. enat (nt - t) > c"])
+  by (auto simp add: less_enat_iff)
 
 lemma fold_Mapping_filter_None: "Mapping.lookup ts as = None \<Longrightarrow>
   Mapping.lookup (fold (\<lambda>(t, X) ts. Mapping.filter
@@ -750,6 +839,19 @@ lemma Mapping_lookup_upd_set: "Mapping.lookup (upd_set m f X) a =
 
 lemma Mapping_upd_set_keys: "Mapping.keys (upd_set m f X) = Mapping.keys m \<union> X"
   by (auto simp add: Mapping_lookup_upd_set dest!: Mapping_keys_dest intro: Mapping_keys_intro)
+
+lift_definition upd_keys_on :: "('a, 'b) mapping \<Rightarrow> ('a \<Rightarrow> 'b \<Rightarrow> 'b) \<Rightarrow> 'a set \<Rightarrow>
+  ('a, 'b) mapping" is
+  "\<lambda>m f X a. case Mapping.lookup m a of Some b \<Rightarrow> Some (if a \<in> X then f a b else b)
+  | None \<Rightarrow> None" .
+
+lemma Mapping_lookup_upd_keys_on: "Mapping.lookup (upd_keys_on m f X) a =
+  (case Mapping.lookup m a of Some b \<Rightarrow> Some (if a \<in> X then f a b else b) | None \<Rightarrow> None)"
+  by (simp add: Mapping.lookup.rep_eq upd_keys_on.rep_eq)
+
+lemma Mapping_upd_keys_sub: "Mapping.keys (upd_keys_on m f X) = Mapping.keys m"
+  by (auto simp add: Mapping_lookup_upd_keys_on dest!: Mapping_keys_dest intro: Mapping_keys_intro
+      split: option.splits)
 
 lemma fold_append_queue_rep: "linearize (fold (\<lambda>x q. append_queue x q) xs q) = linearize q @ xs"
   by (induction xs arbitrary: q) (auto simp add: append_queue_rep)
@@ -1364,31 +1466,1563 @@ lemma valid_result_mmsaux: "valid_mmsaux w n L R aux auxlist \<Longrightarrow>
   result_mmsaux aux = foldr (\<union>) [rel. (t, rel) \<leftarrow> auxlist, left (ivl w) \<le> current w - t] {}"
   using valid_result_mmsaux_unfolded by (cases aux) fast
 
-interpretation default_msaux: msaux valid_mmsaux init_mmsaux filter_mmsaux join_mmsaux add_new_mmsaux result_mmsaux
+interpretation default_msaux: msaux valid_mmsaux init_mmsaux filter_mmsaux join_mmsaux
+  add_new_mmsaux result_mmsaux
   using valid_init_mmsaux valid_filter_mmsaux valid_join_mmsaux valid_add_new_mmsaux
     valid_result_mmsaux by unfold_locales assumption+
 
-(* default until data structure *)
+(* optimized until data structure *)
 
-type_synonym 'a mmuaux = "ts \<times> \<I> \<times> ('a muaux)"
+type_synonym tp = nat
 
-definition valid_mmuaux :: "window \<Rightarrow> nat \<Rightarrow> nat set \<Rightarrow> nat set \<Rightarrow> 'a mmuaux \<Rightarrow> 'a muaux \<Rightarrow> bool" where
-  "valid_mmuaux = (\<lambda>w n L R (nt, I, xs) ys. ivl w = I \<and> current w = nt \<and> xs = ys)"
+type_synonym 'a mmuaux = "tp \<times> nat \<times> ts queue \<times> \<I> \<times> bool \<times> bool list \<times> bool list \<times>
+  ('a tuple, tp) mapping \<times> (tp, ('a tuple, ts + tp) mapping) mapping \<times> 'a table list \<times> nat"
 
-fun init_mmuaux :: "\<I> \<Rightarrow> nat \<Rightarrow> nat set \<Rightarrow> nat set \<Rightarrow> 'a mmuaux" where
-  "init_mmuaux I n L R = (0, I, [])"
+definition tstp_lt :: "ts + tp \<Rightarrow> ts \<Rightarrow> tp \<Rightarrow> bool" where
+  "tstp_lt tstp ts tp = case_sum (\<lambda>ts'. ts' \<le> ts) (\<lambda>tp'. tp' < tp) tstp"
 
-fun add_new_mmuaux :: "bool \<Rightarrow> 'a table \<Rightarrow> 'a table \<Rightarrow> ts \<Rightarrow> 'a mmuaux \<Rightarrow> 'a mmuaux" where
-  "add_new_mmuaux pos rel1 rel2 nt (t, I, xs) = (nt, I, update_until I pos rel1 rel2 nt xs)"
+definition tstp_le :: "ts + tp \<Rightarrow> ts \<Rightarrow> tp \<Rightarrow> bool" where
+  "tstp_le tstp ts tp = case_sum (\<lambda>ts'. ts' \<le> ts) (\<lambda>tp'. tp' \<le> tp) tstp"
+
+definition ts_tp_lt :: "ts \<Rightarrow> tp \<Rightarrow> ts + tp \<Rightarrow> bool" where
+  "ts_tp_lt ts tp tstp = case_sum (\<lambda>ts'. ts \<le> ts') (\<lambda>tp'. tp < tp') tstp"
+
+definition ts_tp_lt' :: "ts \<Rightarrow> tp \<Rightarrow> ts + tp \<Rightarrow> bool" where
+  "ts_tp_lt' ts tp tstp = case_sum (\<lambda>ts'. ts < ts') (\<lambda>tp'. tp \<le> tp') tstp"
+
+definition ts_tp_le :: "ts \<Rightarrow> tp \<Rightarrow> ts + tp \<Rightarrow> bool" where
+  "ts_tp_le ts tp tstp = case_sum (\<lambda>ts'. ts \<le> ts') (\<lambda>tp'. tp \<le> tp') tstp"
+
+fun max_tstp :: "ts + tp \<Rightarrow> ts + tp \<Rightarrow> ts + tp" where
+  "max_tstp (Inl ts) (Inl ts') = Inl (max ts ts')"
+| "max_tstp (Inr tp) (Inr tp') = Inr (max tp tp')"
+| "max_tstp (Inl ts) _ = Inl ts"
+| "max_tstp _ (Inl ts) = Inl ts"
+
+lemma max_tstp_idem: "max_tstp (max_tstp x y) y = max_tstp x y"
+  by (cases x; cases y) auto
+
+lemma max_tstp_idem': "max_tstp x (max_tstp x y) = max_tstp x y"
+  by (cases x; cases y) auto
+
+lemma max_tstp_d_d: "max_tstp d d = d"
+  by (cases d) auto
+
+lemma max_tstpE: "isl tstp \<longleftrightarrow> isl tstp' \<Longrightarrow> (max_tstp tstp tstp' = tstp \<Longrightarrow> P) \<Longrightarrow>
+  (max_tstp tstp tstp' = tstp' \<Longrightarrow> P) \<Longrightarrow> P"
+  apply (cases tstp; cases tstp')
+     apply auto
+  by linarith+
+
+lemma max_tstp_intro: "tstp_lt tstp ts tp \<Longrightarrow> tstp_lt tstp' ts tp \<Longrightarrow> isl tstp \<longleftrightarrow> isl tstp' \<Longrightarrow>
+  tstp_lt (max_tstp tstp tstp') ts tp"
+  by (auto simp add: tstp_lt_def split: sum.splits)
+
+lemma max_tstp_intro': "isl tstp \<longleftrightarrow> isl tstp' \<Longrightarrow>
+  ts_tp_le ts' tp' tstp \<Longrightarrow> ts_tp_le ts' tp' (max_tstp tstp tstp')"
+  by (cases tstp; cases tstp') (auto simp add: ts_tp_le_def tstp_le_def split: sum.splits)
+
+lemma max_tstp_intro'': "isl tstp \<longleftrightarrow> isl tstp' \<Longrightarrow>
+  ts_tp_le ts' tp' tstp' \<Longrightarrow> ts_tp_le ts' tp' (max_tstp tstp tstp')"
+  by (cases tstp; cases tstp') (auto simp add: ts_tp_le_def tstp_le_def split: sum.splits)
+
+lemma max_tstp_intro''': "isl tstp \<longleftrightarrow> isl tstp' \<Longrightarrow>
+  ts_tp_lt' ts' tp' tstp \<Longrightarrow> ts_tp_lt' ts' tp' (max_tstp tstp tstp')"
+  by (cases tstp; cases tstp') (auto simp add: ts_tp_lt'_def tstp_le_def split: sum.splits)
+
+lemma max_tstp_intro'''': "isl tstp \<longleftrightarrow> isl tstp' \<Longrightarrow>
+  ts_tp_lt' ts' tp' tstp' \<Longrightarrow> ts_tp_lt' ts' tp' (max_tstp tstp tstp')"
+  by (cases tstp; cases tstp') (auto simp add: ts_tp_lt'_def tstp_le_def split: sum.splits)
+
+lemma max_tstp_isl: "isl tstp \<longleftrightarrow> isl tstp' \<Longrightarrow> isl (max_tstp tstp tstp') \<longleftrightarrow> isl tstp"
+  by (cases tstp; cases tstp') auto
+
+definition filter_a1_map :: "bool \<Rightarrow> tp \<Rightarrow> ('a tuple, tp) mapping \<Rightarrow> 'a table" where
+  "filter_a1_map pos tp a1_map =
+    {xs \<in> Mapping.keys a1_map. case Mapping.lookup a1_map xs of Some tp' \<Rightarrow>
+    (pos \<longrightarrow> tp' \<le> tp) \<and> (\<not>pos \<longrightarrow> tp \<le> tp')}"
+
+definition filter_a2_map :: "\<I> \<Rightarrow> ts \<Rightarrow> tp \<Rightarrow> (tp, ('a tuple, ts + tp) mapping) mapping \<Rightarrow>
+  'a table" where
+  "filter_a2_map I ts tp a2_map = {xs. \<exists>tp' \<le> tp. (case Mapping.lookup a2_map tp' of Some m \<Rightarrow>
+    (case Mapping.lookup m xs of Some tstp \<Rightarrow> ts_tp_lt' ts tp tstp | _ \<Rightarrow> False)
+    | _ \<Rightarrow> False)}"
+
+fun triple_eq_pair :: "('a \<times> 'b \<times> 'c) \<Rightarrow> ('a \<times> 'd) \<Rightarrow> ('d \<Rightarrow> 'b) \<Rightarrow> ('a \<Rightarrow> 'd \<Rightarrow> 'c) \<Rightarrow> bool" where
+  "triple_eq_pair (t, a1, a2) (ts', tp') f g \<longleftrightarrow> t = ts' \<and> a1 = f tp' \<and> a2 = g ts' tp'"
+
+fun valid_mmuaux' :: "window \<Rightarrow> ts \<Rightarrow> bool \<Rightarrow> nat \<Rightarrow> nat set \<Rightarrow> nat set \<Rightarrow> 'a mmuaux \<Rightarrow> 'a muaux \<Rightarrow>
+  bool" where
+  "valid_mmuaux' w dt b n L R (tp, len, tss, I, pos, maskL, maskR, a1_map, a2_map,
+    done, done_length) auxlist \<longleftrightarrow>
+    L \<subseteq> R \<and> maskL = join_mask n L \<and> maskR = join_mask n R \<and> b = pos \<and>
+    I = ivl w \<and> len \<le> tp \<and>
+    length (linearize tss) = len \<and> sorted (linearize tss) \<and>
+    (\<forall>t \<in> set (linearize tss). t \<le> current w \<and> enat t + right I \<ge> enat (current w)) \<and>
+    table n L (Mapping.keys a1_map) \<and> Mapping.keys a2_map = {tp - len..tp} \<and>
+    (\<forall>xs \<in> Mapping.keys a1_map. case Mapping.lookup a1_map xs of Some tp' \<Rightarrow> tp' < tp) \<and>
+    (\<forall>tp' \<in> Mapping.keys a2_map. case Mapping.lookup a2_map tp' of Some m \<Rightarrow>
+      table n R (Mapping.keys m) \<and>
+      (\<forall>xs \<in> Mapping.keys m. case Mapping.lookup m xs of Some tstp \<Rightarrow>
+      tstp_lt tstp (current w - (left I - 1)) tp \<and> (isl tstp \<longleftrightarrow> left I > 0))) \<and>
+    length done = done_length \<and> length done + len = length auxlist \<and>
+    rev done = map proj_thd (take (length done) auxlist) \<and>
+    (\<forall>x \<in> set (take (length done) auxlist). check_before I dt x) \<and>
+    sorted (map fst auxlist) \<and>
+    list_all2 (\<lambda>x y. triple_eq_pair x y (\<lambda>tp'. filter_a1_map pos tp' a1_map)
+      (\<lambda>ts' tp'. filter_a2_map I ts' tp' a2_map)) (drop (length done) auxlist)
+      (zip (linearize tss) [tp - len..<tp])"
+
+definition valid_mmuaux :: "window \<Rightarrow> bool \<Rightarrow> nat \<Rightarrow> nat set \<Rightarrow> nat set \<Rightarrow> 'a mmuaux \<Rightarrow> 'a muaux \<Rightarrow>
+  bool" where
+  "valid_mmuaux w = valid_mmuaux' w (current w)"
+
+fun eval_step_mmuaux :: "'a mmuaux \<Rightarrow> 'a mmuaux" where
+  "eval_step_mmuaux (tp, len, tss, I, pos, maskL, maskR, a1_map, a2_map,
+    done, done_length) = (case safe_hd tss of (Some ts, tss') \<Rightarrow>
+      (case Mapping.lookup a2_map (tp - len) of Some m \<Rightarrow>
+        let m = Mapping.filter (\<lambda>_ tstp. ts_tp_lt' ts (tp - len) tstp) m;
+        T = Mapping.keys m;
+        a2_map = Mapping.update (tp - len + 1)
+          (case Mapping.lookup a2_map (tp - len + 1) of Some m' \<Rightarrow>
+          Mapping.combine (\<lambda>tstp tstp'. max_tstp tstp tstp') m m') a2_map;
+        a2_map = Mapping.delete (tp - len) a2_map in
+        (tp, len - 1, tl_queue tss', I, pos, maskL, maskR, a1_map, a2_map,
+        T # done, done_length + 1)))"
+
+lemma Mapping_update_keys: "Mapping.keys (Mapping.update a b m) = Mapping.keys m \<union> {a}"
+  by transfer auto
+
+lemma drop_is_Cons_take: "drop n xs = y # ys \<Longrightarrow> take (Suc n) xs = take n xs @ [y]"
+  apply (induction n arbitrary: xs y ys)
+  by auto (metis One_nat_def Suc_eq_plus1 take0 take_Suc_Cons take_add)
+
+lemma list_all2_weaken: "list_all2 f xs ys \<Longrightarrow>
+  (\<And>x y. (x, y) \<in> set (zip xs ys) \<Longrightarrow> f x y \<Longrightarrow> f' x y) \<Longrightarrow> list_all2 f' xs ys"
+  by (induction xs ys rule: list_all2_induct) auto
+
+lemma Mapping_lookup_delete: "Mapping.lookup (Mapping.delete k m) k' =
+  (if k = k' then None else Mapping.lookup m k')"
+  by transfer auto
+
+lemma Mapping_lookup_update: "Mapping.lookup (Mapping.update k v m) k' =
+  (if k = k' then Some v else Mapping.lookup m k')"
+  by transfer auto
+
+lemma hd_le_set: "sorted xs \<Longrightarrow> xs \<noteq> [] \<Longrightarrow> x \<in> set xs \<Longrightarrow> hd xs \<le> x"
+  by (metis eq_iff list.sel(1) set_ConsD sorted.elims(2))
+
+lemma Mapping_lookup_combineE: "Mapping.lookup (Mapping.combine f m m') k = Some v \<Longrightarrow>
+  (Mapping.lookup m k = Some v \<Longrightarrow> P) \<Longrightarrow>
+  (Mapping.lookup m' k = Some v \<Longrightarrow> P) \<Longrightarrow>
+  (\<And>v' v''. Mapping.lookup m k = Some v' \<Longrightarrow> Mapping.lookup m' k = Some v'' \<Longrightarrow>
+  f v' v'' = v \<Longrightarrow> P) \<Longrightarrow> P"
+  unfolding Mapping.lookup_combine
+  by (auto simp add: combine_options_def split: option.splits)
+
+lemma Mapping_keys_filterI: "Mapping.lookup m k = Some v \<Longrightarrow> f k v \<Longrightarrow>
+  k \<in> Mapping.keys (Mapping.filter f m)"
+  by transfer (auto split: option.splits if_splits)
+
+lemma Mapping_keys_filterD: "k \<in> Mapping.keys (Mapping.filter f m) \<Longrightarrow>
+  \<exists>v. Mapping.lookup m k = Some v \<and> f k v"
+  by transfer (auto split: option.splits if_splits)
+
+fun lin_ts_mmuaux :: "'a mmuaux \<Rightarrow> ts list" where
+  "lin_ts_mmuaux (tp, len, tss, I, pos, maskL, maskR, a1_map, a2_map, done, done_length) =
+    linearize tss"
+
+lemma valid_eval_step_mmuaux':
+  assumes "valid_mmuaux' w dt b n L R aux auxlist"
+    "lin_ts_mmuaux aux = ts # tss''" "enat ts + right (ivl w) < dt"
+  shows "valid_mmuaux' w dt b n L R (eval_step_mmuaux aux) auxlist \<and>
+    lin_ts_mmuaux (eval_step_mmuaux aux) = tss''"
+proof -
+  obtain tp len tss I pos maskL maskR a1_map a2_map "done" done_length where aux_def:
+    "aux = (tp, len, tss, I, pos, maskL, maskR, a1_map, a2_map, done, done_length)"
+    by (cases aux) auto
+  then obtain tss' where safe_hd_eq: "safe_hd tss = (Some ts, tss')"
+    using assms(2) safe_hd_rep case_optionE
+    by (cases "safe_hd tss") fastforce
+  note valid_before = assms(1)[unfolded aux_def]
+  have I_ivl_w: "I = ivl w"
+    using valid_before by auto
+  have lin_tss_not_Nil: "linearize tss \<noteq> []"
+    using safe_hd_rep[OF safe_hd_eq] by auto
+  have ts_hd: "ts = hd (linearize tss)"
+    using safe_hd_rep[OF safe_hd_eq] by auto
+  have lin_tss': "linearize tss' = linearize tss"
+    using safe_hd_rep[OF safe_hd_eq] by auto
+  have tss'_not_empty: "\<not>is_empty tss'"
+    using is_empty_alt[of tss'] lin_tss_not_Nil unfolding lin_tss' by auto
+  have len_pos: "len > 0"
+    using lin_tss_not_Nil valid_before by auto
+  have a2_map_keys: "Mapping.keys a2_map = {tp - len..tp}"
+    using valid_before by auto
+  have len_tp: "len \<le> tp"
+    using valid_before by auto
+  have tp_minus_keys: "tp - len \<in> Mapping.keys a2_map"
+    using a2_map_keys by auto
+  have tp_minus_keys': "tp - len + 1 \<in> Mapping.keys a2_map"
+    using a2_map_keys len_pos len_tp by auto
+  obtain m where m_def: "Mapping.lookup a2_map (tp - len) = Some m"
+    using tp_minus_keys by (auto dest: Mapping_keys_dest)
+  have "table n R (Mapping.keys m)"
+    "(\<forall>xs \<in> Mapping.keys m. case Mapping.lookup m xs of Some tstp \<Rightarrow>
+    tstp_lt tstp (current w - (left I - 1)) tp \<and> (isl tstp \<longleftrightarrow> left I > 0))"
+    using tp_minus_keys m_def valid_before
+    unfolding valid_mmuaux'.simps by fastforce+
+  then have m_inst: "table n R (Mapping.keys m)"
+    "\<And>xs tstp. Mapping.lookup m xs = Some tstp \<Longrightarrow>
+    tstp_lt tstp (current w - (left I - 1)) tp \<and> (isl tstp \<longleftrightarrow> left I > 0)"
+    using Mapping_keys_intro by fastforce+
+  have m_inst_isl: "\<And>xs tstp. Mapping.lookup m xs = Some tstp \<Longrightarrow> isl tstp \<longleftrightarrow> left I > 0"
+    using m_inst(2) by fastforce
+  obtain m' where m'_def: "Mapping.lookup a2_map (tp - len + 1) = Some m'"
+    using tp_minus_keys' by (auto dest: Mapping_keys_dest)
+  have "table n R (Mapping.keys m')"
+    "(\<forall>xs \<in> Mapping.keys m'. case Mapping.lookup m' xs of Some tstp \<Rightarrow>
+    tstp_lt tstp (current w - (left I - 1)) tp \<and> (isl tstp \<longleftrightarrow> left I > 0))"
+    using tp_minus_keys' m'_def valid_before
+    unfolding valid_mmuaux'.simps by fastforce+
+  then have m'_inst: "table n R (Mapping.keys m')"
+    "\<And>xs tstp. Mapping.lookup m' xs = Some tstp \<Longrightarrow>
+    tstp_lt tstp (current w - (left I - 1)) tp \<and> (isl tstp \<longleftrightarrow> left I > 0)"
+    using Mapping_keys_intro by fastforce+
+  have m'_inst_isl: "\<And>xs tstp. Mapping.lookup m' xs = Some tstp \<Longrightarrow> isl tstp \<longleftrightarrow> left I > 0"
+    using m'_inst(2) by fastforce  
+  define m_upd where "m_upd = Mapping.filter (\<lambda>_ tstp. ts_tp_lt' ts (tp - len) tstp) m"
+  define T where "T = Mapping.keys m_upd"
+  define mc where "mc = Mapping.combine (\<lambda>tstp tstp'. max_tstp tstp tstp') m_upd m'"
+  define a2_map' where "a2_map' = Mapping.update (tp - len + 1) mc a2_map"
+  define a2_map'' where "a2_map'' = Mapping.delete (tp - len) a2_map'"
+  have m_upd_lookup: "\<And>xs tstp. Mapping.lookup m_upd xs = Some tstp \<Longrightarrow>
+    tstp_lt tstp (current w - (left I - 1)) tp \<and> (isl tstp \<longleftrightarrow> left I > 0)"
+    unfolding m_upd_def Mapping.lookup_filter
+    using m_inst(2) by (auto split: option.splits if_splits)
+  have mc_lookup: "\<And>xs tstp. Mapping.lookup mc xs = Some tstp \<Longrightarrow>
+    tstp_lt tstp (current w - (left I - 1)) tp \<and> (isl tstp \<longleftrightarrow> left I > 0)"
+    unfolding mc_def Mapping.lookup_combine
+    using m_upd_lookup m'_inst(2)
+    by (auto simp add: combine_options_def max_tstp_isl intro: max_tstp_intro split: option.splits)
+  have mc_keys: "Mapping.keys mc \<subseteq> Mapping.keys m \<union> Mapping.keys m'"
+    unfolding mc_def Mapping.keys_combine m_upd_def
+    using Mapping.keys_filter by fastforce
+  have tp_len_assoc: "tp - len + 1 = tp - (len - 1)"
+    using len_pos len_tp by auto
+  have a2_map''_keys: "Mapping.keys a2_map'' = {tp - (len - 1)..tp}"
+    unfolding a2_map''_def a2_map'_def Mapping.keys_delete Mapping_update_keys a2_map_keys
+    using tp_len_assoc by auto
+  have lin_tss_Cons: "linearize tss = ts # linearize (tl_queue tss')"
+    using lin_tss_not_Nil
+    by (auto simp add: tl_queue_rep[OF tss'_not_empty] lin_tss' ts_hd)
+  have tp_len_tp_unfold: "[tp - len..<tp] = (tp - len) # [tp - (len - 1)..<tp]"
+    unfolding tp_len_assoc[symmetric]
+    using len_pos len_tp Suc_diff_le upt_conv_Cons by auto
+  have id: "\<And>x. x \<in> {tp - (len - 1) + 1..tp} \<Longrightarrow>
+    Mapping.lookup a2_map'' x = Mapping.lookup a2_map x"
+    unfolding a2_map''_def a2_map'_def Mapping_lookup_delete Mapping_lookup_update tp_len_assoc
+    using len_tp by auto
+  have list_all2: "list_all2 (\<lambda>x y. triple_eq_pair x y (\<lambda>tp'. filter_a1_map pos tp' a1_map)
+    (\<lambda>ts' tp'. filter_a2_map I ts' tp' a2_map))
+    (drop (length done) auxlist) (zip (linearize tss) [tp - len..<tp])"
+    using valid_before by auto
+  obtain hd_aux tl_aux where aux_split: "drop (length done) auxlist = hd_aux # tl_aux"
+    "case hd_aux of (t, a1, a2) \<Rightarrow> (t, a1, a2) =
+    (ts, filter_a1_map pos (tp - len) a1_map, filter_a2_map I ts (tp - len) a2_map)"
+    and list_all2': "list_all2 (\<lambda>x y. triple_eq_pair x y (\<lambda>tp'. filter_a1_map pos tp' a1_map)
+      (\<lambda>ts' tp'. filter_a2_map I ts' tp' a2_map)) tl_aux
+      (zip (linearize (tl_queue tss')) [tp - (len - 1)..<tp])"
+    using list_all2[unfolded lin_tss_Cons tp_len_tp_unfold zip_Cons_Cons list_all2_Cons2] by auto
+  have lookup''_tp_minus: "Mapping.lookup a2_map'' (tp - (len - 1)) = Some mc"
+    unfolding a2_map''_def a2_map'_def Mapping_lookup_delete Mapping_lookup_update
+      tp_len_assoc[symmetric]
+    using len_tp by auto
+  have filter_a2_map_cong: "\<And>ts' tp'. ts' \<in> set (linearize tss) \<Longrightarrow>
+    tp' \<in> {tp - (len - 1)..<tp} \<Longrightarrow> filter_a2_map I ts' tp' a2_map =
+    filter_a2_map I ts' tp' a2_map''"
+  proof (rule set_eqI, rule iffI)
+    fix ts' tp' xs
+    assume assms: "ts' \<in> set (linearize tss)"
+      "tp' \<in> {tp - (len - 1)..<tp}" "xs \<in> filter_a2_map I ts' tp' a2_map"
+    obtain tp_bef m_bef tstp where defs: "tp_bef \<le> tp'" "Mapping.lookup a2_map tp_bef = Some m_bef"
+      "Mapping.lookup m_bef xs = Some tstp" "ts_tp_lt' ts' tp' tstp"
+      using assms(3)[unfolded filter_a2_map_def]
+      by (fastforce split: option.splits)
+    have ts_le_ts': "ts \<le> ts'"
+      using hd_le_set[OF _ lin_tss_not_Nil assms(1)] valid_before
+      unfolding ts_hd by auto
+    have tp_bef_in: "tp_bef \<in> {tp - len..tp}"
+      using defs(2) valid_before by (auto intro!: Mapping_keys_intro)
+    have tp_minus_le: "tp - (len - 1) \<le> tp'"
+      using assms(2) by auto
+    show "xs \<in> filter_a2_map I ts' tp' a2_map''"
+    proof (cases "tp_bef \<le> tp - (len - 1)")
+      case True
+      show ?thesis
+      proof (cases "tp_bef = tp - len")
+        case True
+        have m_bef_m: "m_bef = m"
+          using defs(2) m_def
+          unfolding True by auto
+        have "Mapping.lookup m_upd xs = Some tstp"
+          using defs(3,4) assms(2) ts_le_ts' unfolding m_bef_m m_upd_def
+          by (auto simp add: Mapping.lookup_filter ts_tp_lt'_def intro: Mapping_keys_intro
+              split: sum.splits)
+        then have "case Mapping.lookup mc xs of None \<Rightarrow> False | Some tstp \<Rightarrow>
+          ts_tp_lt' ts' tp' tstp"
+          unfolding mc_def Mapping.lookup_combine
+          using m'_inst(2) m_upd_lookup
+          by (auto simp add: combine_options_def defs(4) intro!: max_tstp_intro'''
+              dest: Mapping_keys_dest split: option.splits)
+        then show ?thesis
+          using lookup''_tp_minus tp_minus_le defs
+          unfolding m_bef_m filter_a2_map_def by (auto split: option.splits)
+      next
+        case False
+        then have "tp_bef = tp - (len - 1)"
+          using True tp_bef_in by auto
+        then have m_bef_m: "m_bef = m'"
+          using defs(2) m'_def
+          unfolding tp_len_assoc by auto
+        have "case Mapping.lookup mc xs of None \<Rightarrow> False | Some tstp \<Rightarrow>
+          ts_tp_lt' ts' tp' tstp"
+          unfolding mc_def Mapping.lookup_combine
+          using m'_inst(2) m_upd_lookup defs(3)[unfolded m_bef_m]
+          by (auto simp add: combine_options_def defs(4) intro!: max_tstp_intro''''
+              dest: Mapping_keys_dest split: option.splits)
+        then show ?thesis
+          using lookup''_tp_minus tp_minus_le defs
+          unfolding m_bef_m filter_a2_map_def by (auto split: option.splits)
+      qed
+    next
+      case False
+      then have "Mapping.lookup a2_map'' tp_bef = Mapping.lookup a2_map tp_bef"
+        using id tp_bef_in len_tp by auto
+      then show ?thesis
+        unfolding filter_a2_map_def
+        using defs by auto
+    qed
+  next
+    fix ts' tp' xs
+    assume assms: "ts' \<in> set (linearize tss)" "tp' \<in> {tp - (len - 1)..<tp}"
+      "xs \<in> filter_a2_map I ts' tp' a2_map''"
+    obtain tp_bef m_bef tstp where defs: "tp_bef \<le> tp'"
+      "Mapping.lookup a2_map'' tp_bef = Some m_bef"
+      "Mapping.lookup m_bef xs = Some tstp" "ts_tp_lt' ts' tp' tstp"
+      using assms(3)[unfolded filter_a2_map_def]
+      by (fastforce split: option.splits)
+    have ts_le_ts': "ts \<le> ts'"
+      using hd_le_set[OF _ lin_tss_not_Nil assms(1)] valid_before
+      unfolding ts_hd by auto
+    have tp_bef_in: "tp_bef \<in> {tp - (len - 1)..tp}"
+      using defs(2) a2_map''_keys by (auto intro!: Mapping_keys_intro)
+    have tp_minus_le: "tp - len \<le> tp'" "tp - (len - 1) \<le> tp'"
+      using assms(2) by auto
+    show "xs \<in> filter_a2_map I ts' tp' a2_map"
+    proof (cases "tp_bef = tp - (len - 1)")
+      case True
+      have m_beg_mc: "m_bef = mc"
+        using defs(2)
+        unfolding True a2_map''_def a2_map'_def tp_len_assoc Mapping_lookup_delete
+          Mapping.lookup_update
+        by (auto split: if_splits)
+      show ?thesis
+        using defs(3)[unfolded m_beg_mc mc_def]
+      proof (rule Mapping_lookup_combineE)
+        assume lassm: "Mapping.lookup m_upd xs = Some tstp"
+        then show "xs \<in> filter_a2_map I ts' tp' a2_map"
+          unfolding m_upd_def Mapping.lookup_filter
+          using m_def tp_minus_le(1) defs
+          by (auto simp add: filter_a2_map_def split: option.splits if_splits)
+      next
+        assume lassm: "Mapping.lookup m' xs = Some tstp"
+        then show "xs \<in> filter_a2_map I ts' tp' a2_map"
+          using m'_def defs(4) tp_minus_le defs
+          unfolding filter_a2_map_def tp_len_assoc
+          by auto
+      next
+        fix v' v''
+        assume lassms: "Mapping.lookup m_upd xs = Some v'" "Mapping.lookup m' xs = Some v''"
+          "max_tstp v' v'' = tstp"
+        show "xs \<in> filter_a2_map I ts' tp' a2_map"
+        proof (rule max_tstpE)
+          show "isl v' = isl v''"
+            using lassms(1,2) m_upd_lookup m'_inst(2)
+            by auto
+        next
+          assume "max_tstp v' v'' = v'"
+          then show "xs \<in> filter_a2_map I ts' tp' a2_map"
+            using lassms(1,3) m_def defs tp_minus_le(1)
+            unfolding tp_len_assoc m_upd_def Mapping.lookup_filter
+            by (auto simp add: filter_a2_map_def split: option.splits if_splits)
+        next
+          assume "max_tstp v' v'' = v''"
+          then show "xs \<in> filter_a2_map I ts' tp' a2_map"
+            using lassms(2,3) m'_def defs tp_minus_le(2)
+            unfolding tp_len_assoc
+            by (auto simp add: filter_a2_map_def)
+        qed
+      qed
+    next
+      case False
+      then have "Mapping.lookup a2_map'' tp_bef = Mapping.lookup a2_map tp_bef"
+        using id tp_bef_in by auto
+      then show ?thesis
+        unfolding filter_a2_map_def
+        using defs by auto (metis option.simps(5))
+    qed
+  qed
+  have set_tl_tss': "set (linearize (tl_queue tss')) \<subseteq> set (linearize tss)"
+    unfolding tl_queue_rep[OF tss'_not_empty] lin_tss_Cons by auto
+  have list_all2'': "list_all2 (\<lambda>x y. triple_eq_pair x y (\<lambda>tp'. filter_a1_map pos tp' a1_map)
+      (\<lambda>ts' tp'. filter_a2_map I ts' tp' a2_map'')) tl_aux
+      (zip (linearize (tl_queue tss')) [tp - (len - 1)..<tp])"
+    apply (rule list_all2_weaken[OF list_all2'])
+    using filter_a2_map_cong set_tl_tss' by (auto elim!: in_set_zipE split: prod.splits)
+  have lookup'': "\<forall>tp' \<in> Mapping.keys a2_map''. case Mapping.lookup a2_map'' tp' of Some m \<Rightarrow>
+    table n R (Mapping.keys m) \<and> (\<forall>xs \<in> Mapping.keys m. case Mapping.lookup m xs of Some tstp \<Rightarrow>
+    tstp_lt tstp (current w - (left I - 1)) tp \<and> isl tstp = (0 < left I))"
+  proof (rule ballI)
+    fix tp'
+    assume assm: "tp' \<in> Mapping.keys a2_map''"
+    then obtain f where f_def: "Mapping.lookup a2_map'' tp' = Some f"
+      by (auto dest: Mapping_keys_dest)
+    have tp'_in: "tp' \<in> {tp - (len - 1)..tp}"
+      using assm unfolding a2_map''_keys .
+    then have tp'_in_keys: "tp' \<in> Mapping.keys a2_map"
+      using valid_before by auto
+    have "table n R (Mapping.keys f) \<and>
+      (\<forall>xs \<in> Mapping.keys f. case Mapping.lookup f xs of Some tstp \<Rightarrow>
+      tstp_lt tstp (current w - (left I - 1)) tp \<and> isl tstp = (0 < left I))"
+    proof (cases "tp' = tp - (len - 1)")
+      case True
+      then have f_mc: "f = mc"
+        using f_def
+        unfolding a2_map''_def a2_map'_def Mapping_lookup_delete Mapping_lookup_update tp_len_assoc
+        by (auto split: if_splits)
+      have "table n R (Mapping.keys f)"
+        unfolding f_mc
+        using mc_keys m_def m'_def m_inst m'_inst
+        by (auto simp add: table_def)
+      moreover have "\<forall>xs \<in> Mapping.keys f. case Mapping.lookup f xs of Some tstp \<Rightarrow>
+        tstp_lt tstp (current w - (left I - 1)) tp \<and> isl tstp = (0 < left I)"
+        using assm Mapping.keys_filter m_inst(2) m_inst_isl m'_inst(2) m'_inst_isl max_tstp_isl
+        unfolding f_mc mc_def Mapping.lookup_combine
+        by (auto simp add: combine_options_def m_upd_def Mapping.lookup_filter
+            intro!: max_tstp_intro Mapping_keys_intro dest!: Mapping_keys_dest
+            split: option.splits)
+      ultimately show ?thesis
+        by auto
+    next
+      case False
+      have "Mapping.lookup a2_map tp' = Some f"
+        using tp'_in id[of tp'] f_def False by auto
+      then show ?thesis
+        using tp'_in_keys valid_before
+        unfolding valid_mmuaux'.simps by fastforce
+    qed
+    then show "case Mapping.lookup a2_map'' tp' of Some m \<Rightarrow>
+      table n R (Mapping.keys m) \<and> (\<forall>xs \<in> Mapping.keys m. case Mapping.lookup m xs of Some tstp \<Rightarrow>
+      tstp_lt tstp (current w - (left I - 1)) tp \<and> isl tstp = (0 < left I))"
+      using f_def by auto
+  qed
+  have tl_aux_def: "tl_aux = drop (length done + 1) auxlist"
+    using aux_split(1) by (metis Suc_eq_plus1 add_Suc drop0 drop_Suc_Cons drop_drop)
+  have T_eq: "T = filter_a2_map I ts (tp - len) a2_map"
+  proof (rule set_eqI, rule iffI)
+    fix xs
+    assume "xs \<in> filter_a2_map I ts (tp - len) a2_map"
+    then obtain tp_bef m_bef tstp where defs: "tp_bef \<le> tp - len"
+      "Mapping.lookup a2_map tp_bef = Some m_bef"
+      "Mapping.lookup m_bef xs = Some tstp" "ts_tp_lt' ts (tp - len) tstp"
+      by (fastforce simp add: filter_a2_map_def split: option.splits)
+    then have tp_bef_minus: "tp_bef = tp - len"
+      using valid_before Mapping_keys_intro by force
+    have m_bef_m: "m_bef = m"
+      using defs(2) m_def
+      unfolding tp_bef_minus by auto
+    show "xs \<in> T"
+      using defs
+      unfolding T_def m_upd_def m_bef_m
+      by (auto intro: Mapping_keys_filterI Mapping_keys_intro)
+  next
+    fix xs
+    assume "xs \<in> T"
+    then show "xs \<in> filter_a2_map I ts (tp - len) a2_map"
+      using m_def Mapping.keys_filter
+      unfolding T_def m_upd_def filter_a2_map_def
+      by (auto simp add: filter_a2_map_def dest!: Mapping_keys_filterD split: if_splits)
+  qed
+  have min_auxlist_done: "min (length auxlist) (length done) = length done"
+    using valid_before by auto
+  then have "\<forall>x \<in> set (take (length done) auxlist). check_before I dt x"
+    "rev done = map proj_thd (take (length done) auxlist)"
+    using valid_before by auto
+  then have list_all': "(\<forall>x \<in> set (take (length (T # done)) auxlist). check_before I dt x)"
+    "rev (T # done) = map proj_thd (take (length (T # done)) auxlist)"
+    using drop_is_Cons_take[OF aux_split(1)] aux_split(2) assms(3)[unfolded I_ivl_w[symmetric]]
+    by (auto simp add: T_eq)
+  have eval_step_mmuaux_eq: "eval_step_mmuaux (tp, len, tss, I, pos, maskL, maskR, a1_map, a2_map,
+    done, done_length) = (tp, len - 1, tl_queue tss', I, pos, maskL, maskR, a1_map, a2_map'',
+    T # done, done_length + 1)"
+    using safe_hd_eq m_def m'_def m_upd_def T_def mc_def a2_map'_def a2_map''_def
+    by (auto simp add: Let_def)
+  have "lin_ts_mmuaux (eval_step_mmuaux aux) = tss''"
+    using lin_tss_Cons assms(2) unfolding aux_def eval_step_mmuaux_eq by auto
+  then show ?thesis
+    using valid_before a2_map''_keys sorted_tl list_all' lookup'' list_all2''
+    unfolding eval_step_mmuaux_eq valid_mmuaux'.simps tl_aux_def aux_def
+    using lin_tss_not_Nil safe_hd_eq len_pos
+    by (auto simp add: list.set_sel(2) lin_tss' tl_queue_rep[OF tss'_not_empty] min_auxlist_done)
+qed
+
+lemma done_empty_valid_mmuaux'_intro:
+  assumes "valid_mmuaux' w dt b n L R
+    (tp, len, tss, I, pos, maskL, maskR, a1_map, a2_map, done, done_length) auxlist"
+  shows "valid_mmuaux' w dt' b n L R
+    (tp, len, tss, I, pos, maskL, maskR, a1_map, a2_map, [], 0)
+    (drop (length done) auxlist)"
+  using assms sorted_drop by (auto simp add: drop_map[symmetric])
+
+lemma valid_mmuaux'_mono:
+  assumes "valid_mmuaux' w dt b n L R aux auxlist" "dt \<le> dt'"
+  shows "valid_mmuaux' w dt' b n L R aux auxlist"
+  using assms less_le_trans by (cases aux) fastforce
+
+lemma valid_foldl_eval_step_mmuaux':
+  assumes valid_before: "valid_mmuaux' w dt b n L R aux auxlist"
+    "lin_ts_mmuaux aux = tss @ tss'"
+    "\<And>ts. ts \<in> set (take (length tss) (lin_ts_mmuaux aux)) \<Longrightarrow> enat ts + right (ivl w) < dt"
+  shows "valid_mmuaux' w dt b n L R (foldl (\<lambda>aux _. eval_step_mmuaux aux) aux tss) auxlist \<and>
+    lin_ts_mmuaux (foldl (\<lambda>aux _. eval_step_mmuaux aux) aux tss) = tss'"
+  using assms
+proof (induction tss arbitrary: aux)
+  case (Cons ts tss)
+  have app_ass: "lin_ts_mmuaux aux = ts # (tss @ tss')"
+    using Cons(3) by auto
+  have "enat ts + right (ivl w) < dt"
+    using Cons by auto
+  then have valid_step: "valid_mmuaux' w dt b n L R (eval_step_mmuaux aux) auxlist"
+    "lin_ts_mmuaux (eval_step_mmuaux aux) = tss @ tss'"
+    using valid_eval_step_mmuaux'[OF Cons(2) app_ass] by auto
+  show ?case
+    using Cons(1)[OF valid_step] valid_step Cons(4) app_ass by auto
+qed auto
+
+lemma sorted_dropWhile_filter: "sorted xs \<Longrightarrow> dropWhile (\<lambda>t. enat t + right I < enat nt) xs =
+  filter (\<lambda>t. \<not>enat t + right I < enat nt) xs"
+proof (induction xs)
+  case (Cons x xs)
+  then show ?case
+  proof (cases "enat x + right I < enat nt")
+    case False
+    then have neg: "enat x + right I \<ge> enat nt"
+      by auto
+    have "\<And>z. z \<in> set xs \<Longrightarrow> \<not>enat z + right I < enat nt"
+    proof -
+      fix z
+      assume "z \<in> set xs"
+      then have "enat z + right I \<ge> enat x + right I"
+        using Cons by auto
+      with neg have "enat z + right I \<ge> enat nt"
+        using dual_order.trans by blast
+      then show "\<not>enat z + right I < enat nt"
+        by auto
+    qed
+    with False show ?thesis
+      using filter_empty_conv by auto
+  qed auto
+qed auto
+
+fun shift_mmuaux :: "ts \<Rightarrow> 'a mmuaux \<Rightarrow> 'a mmuaux" where
+  "shift_mmuaux nt (tp, len, tss, I, pos, maskL, maskR, a1_map, a2_map, done, done_length) =
+    (let tss_list = linearize (takeWhile_queue (\<lambda>t. enat t + right I < enat nt) tss) in
+    foldl (\<lambda>aux _. eval_step_mmuaux aux) (tp, len, tss, I, pos, maskL, maskR,
+      a1_map, a2_map, done, done_length) tss_list)"
+
+lemma valid_shift_mmuaux':
+  assumes "valid_mmuaux' w (current w) b n L R aux auxlist" "nt \<ge> current w"
+  shows "valid_mmuaux' w nt b n L R (shift_mmuaux nt aux) auxlist \<and>
+    (\<forall>ts \<in> set (lin_ts_mmuaux (shift_mmuaux nt aux)). \<not>enat ts + right (ivl w) < nt)"
+proof -
+  have valid_folded: "valid_mmuaux' w nt b n L R aux auxlist"
+    using assms(1,2) valid_mmuaux'_mono unfolding valid_mmuaux_def by blast
+  obtain tp len tss I pos maskL maskR a1_map a2_map "done" done_length where aux_def:
+    "aux = (tp, len, tss, I, pos, maskL, maskR, a1_map, a2_map, done, done_length)"
+    by (cases aux) auto
+  have b_pos: "b = pos"
+    using valid_folded unfolding aux_def by auto
+  note valid_before = valid_folded[unfolded aux_def this]
+  have I_ivl_w: "I = ivl w"
+    using valid_before by auto
+  define tss_list where "tss_list =
+    linearize (takeWhile_queue (\<lambda>t. enat t + right I < enat nt) tss)"
+  have tss_list_takeWhile: "tss_list = takeWhile (\<lambda>t. enat t + right I < enat nt) (linearize tss)"
+    using tss_list_def unfolding takeWhile_queue_rep .
+  then obtain tss_list' where tss_list'_def: "linearize tss = tss_list @ tss_list'"
+    "tss_list' = dropWhile (\<lambda>t. enat t + right I < enat nt) (linearize tss)"
+    by auto
+  obtain tp' len' tss' I' pos' maskL' maskR' a1_map' a2_map' "done'" done_length' where
+    foldl_aux_def: "(tp', len', tss', I', pos', maskL', maskR', a1_map', a2_map',
+      done', done_length') = foldl (\<lambda>aux _. eval_step_mmuaux aux) aux tss_list"
+    by (cases "foldl (\<lambda>aux _. eval_step_mmuaux aux) aux tss_list") auto
+  have lin_tss_aux: "lin_ts_mmuaux aux = linearize tss"
+    unfolding aux_def by auto
+  have "take (length tss_list) (lin_ts_mmuaux aux) = tss_list"
+    unfolding lin_tss_aux using tss_list'_def(1) by auto
+  then have valid_foldl: "valid_mmuaux' w nt pos n L R
+    (foldl (\<lambda>aux _. eval_step_mmuaux aux) aux tss_list) auxlist"
+    "lin_ts_mmuaux (foldl (\<lambda>aux _. eval_step_mmuaux aux) aux tss_list) = tss_list'"
+    using valid_foldl_eval_step_mmuaux'[OF valid_before[folded aux_def], unfolded lin_tss_aux,
+      OF tss_list'_def(1)] tss_list_takeWhile I_ivl_w set_takeWhileD
+    unfolding lin_tss_aux by fastforce+
+  have shift_mmuaux_eq: "shift_mmuaux nt aux = foldl (\<lambda>aux _. eval_step_mmuaux aux) aux tss_list"
+    using tss_list_def unfolding aux_def by auto
+  have "\<And>ts. ts \<in> set tss_list' \<Longrightarrow> \<not>enat ts + right (ivl w) < nt"
+    using sorted_dropWhile_filter tss_list'_def(2) valid_before unfolding I_ivl_w by auto
+  then show ?thesis
+    using valid_foldl(1)[unfolded shift_mmuaux_eq[symmetric] b_pos[symmetric]]
+    unfolding valid_foldl(2)[unfolded shift_mmuaux_eq[symmetric]] by auto
+qed
+
+lift_definition upd_set' :: "('a, 'b) mapping \<Rightarrow> 'b \<Rightarrow> ('b \<Rightarrow> 'b) \<Rightarrow> 'a set \<Rightarrow> ('a, 'b) mapping" is
+  "\<lambda>m d f X a. (if a \<in> X then (case Mapping.lookup m a of Some b \<Rightarrow> Some (f b) | None \<Rightarrow> Some d)
+    else Mapping.lookup m a)" .
+
+lemma upd_set'_lookup: "Mapping.lookup (upd_set' m d f X) a = (if a \<in> X then
+  (case Mapping.lookup m a of Some b \<Rightarrow> Some (f b) | None \<Rightarrow> Some d) else Mapping.lookup m a)"
+  by (simp add: lookup.rep_eq upd_set'.rep_eq)
+
+lemma upd_set'_keys: "Mapping.keys (upd_set' m d f X) = Mapping.keys m \<union> X"
+  by (auto simp add: upd_set'_lookup intro!: Mapping_keys_intro
+      dest!: Mapping_keys_dest split: option.splits)
+
+lift_definition upd_nested :: "('a, ('b, 'c) mapping) mapping \<Rightarrow>
+  'c \<Rightarrow> ('c \<Rightarrow> 'c) \<Rightarrow> ('a \<times> 'b) set \<Rightarrow> ('a, ('b, 'c) mapping) mapping" is
+  "\<lambda>m d f X a. case Mapping.lookup m a of Some m' \<Rightarrow> Some (upd_set' m' d f {b. (a, b) \<in> X})
+  | None \<Rightarrow> if a \<in> fst ` X then Some (upd_set' Mapping.empty d f {b. (a, b) \<in> X}) else None" .
+
+lemma upd_nested_lookup: "Mapping.lookup (upd_nested m d f X) a =
+  (case Mapping.lookup m a of Some m' \<Rightarrow> Some (upd_set' m' d f {b. (a, b) \<in> X})
+  | None \<Rightarrow> if a \<in> fst ` X then Some (upd_set' Mapping.empty d f {b. (a, b) \<in> X}) else None)"
+  by (simp add: lookup.abs_eq upd_nested.abs_eq)
+
+lemma upd_nested_keys: "Mapping.keys (upd_nested m d f X) = Mapping.keys m \<union> fst ` X"
+  by (auto simp add: upd_nested_lookup Domain.DomainI fst_eq_Domain intro!: Mapping_keys_intro
+      dest!: Mapping_keys_dest split: option.splits)
+
+fun add_new_mmuaux :: "'a table \<Rightarrow> 'a table \<Rightarrow> ts \<Rightarrow> 'a mmuaux \<Rightarrow> 'a mmuaux" where
+  "add_new_mmuaux rel1 rel2 nt aux =
+    (let (tp, len, tss, I, pos, maskL, maskR, a1_map, a2_map, done, done_length) =
+    shift_mmuaux nt aux;
+    new_tstp = (if left I = 0 then Inr tp else Inl (nt - (left I - 1)));
+    tmp = \<Union>((\<lambda>as. case Mapping.lookup a1_map (proj_tuple maskL as) of None \<Rightarrow>
+      (if \<not>pos then {(tp - len, as)} else {})
+      | Some tp' \<Rightarrow> if pos then {(max (tp - len) tp', as)}
+      else {(max (tp - len) (tp' + 1), as)}) ` rel2) \<union> (if left I = 0 then {tp} \<times> rel2 else {});
+    a2_map = Mapping.update (tp + 1) Mapping.empty
+      (upd_nested a2_map new_tstp (max_tstp new_tstp) tmp);
+    a1_map = (if pos then Mapping.filter (\<lambda>as _. as \<in> rel1)
+      (upd_set a1_map (\<lambda>_. tp) (rel1 - Mapping.keys a1_map)) else upd_set a1_map (\<lambda>_. tp) rel1);
+    tss = append_queue nt tss in
+    (tp + 1, len + 1, tss, I, pos, maskL, maskR, a1_map, a2_map, done, done_length))"
+
+lemma fst_case: "(\<lambda>x. fst (case x of (t, a1, a2) \<Rightarrow> (t, y t a1 a2, z t a1 a2))) = fst"
+  by auto
+
+lemma list_all2_zip: "list_all2 (\<lambda>x y. triple_eq_pair x y f g) xs (zip ys zs) \<Longrightarrow>
+  (\<And>y. y \<in> set ys \<Longrightarrow> Q y) \<Longrightarrow> x \<in> set xs \<Longrightarrow> Q (fst x)"
+  apply (induction xs "zip ys zs" arbitrary: ys zs rule: list_all2_induct)
+   apply auto
+   apply (metis in_set_zipE list.set_intros(1))
+  by (metis in_mono set_subset_Cons zip_eq_ConsE)
+
+lemma list_appendE: "xs = ys @ zs \<Longrightarrow> x \<in> set xs \<Longrightarrow>
+  (x \<in> set ys \<Longrightarrow> P) \<Longrightarrow> (x \<in> set zs \<Longrightarrow> P) \<Longrightarrow> P"
+  by auto
+
+lemma take_length_takeWhile: "length xs \<le> length ys \<Longrightarrow>
+  (\<And>y. y \<in> set (take (length xs) ys) \<Longrightarrow> P y) \<Longrightarrow>
+  (\<And>y. y \<in> set (drop (length xs) ys) \<Longrightarrow> \<not>P y) \<Longrightarrow>
+  take (length xs) ys = takeWhile P ys"
+  apply (induction xs arbitrary: ys)
+   apply auto
+   apply (metis list.set_sel(1) takeWhile.simps(1) takeWhile_hd_tl)
+  by (metis Suc_le_eq drop_eq_Nil hd_drop_conv_nth id_take_nth_drop list.set_sel(1)
+      not_less_eq_eq takeWhile_eq_all_conv takeWhile_tail take_Suc_conv_app_nth)
+
+lemma valid_add_new_mmuaux:
+  assumes valid_before: "valid_mmuaux w b n L R aux auxlist"
+    and tabs: "table n L rel1" "table n R rel2"
+    and nt_mono: "nt \<ge> current w"
+    and new_window: "w' = w\<lparr>current := nt\<rparr>"
+  shows "valid_mmuaux w' b n L R (add_new_mmuaux rel1 rel2 nt aux)
+    (update_until (ivl w) b rel1 rel2 nt auxlist)"
+proof -
+  have valid_folded: "valid_mmuaux' w nt b n L R aux auxlist"
+    using assms(1,4) valid_mmuaux'_mono unfolding valid_mmuaux_def by blast
+  obtain tp len tss I pos maskL maskR a1_map a2_map "done" done_length where shift_aux_def:
+    "shift_mmuaux nt aux = (tp, len, tss, I, pos, maskL, maskR, a1_map, a2_map, done, done_length)"
+    by (cases "shift_mmuaux nt aux") auto
+  have valid_shift_aux: "valid_mmuaux' w nt b n L R (tp, len, tss, I, pos, maskL, maskR,
+    a1_map, a2_map, done, done_length) auxlist"
+    "\<And>ts. ts \<in> set (linearize tss) \<Longrightarrow> \<not>enat ts + right (ivl w) < enat nt"
+    using valid_shift_mmuaux'[OF assms(1)[unfolded valid_mmuaux_def] assms(4)]
+    unfolding shift_aux_def by auto
+  have b_pos: "b = pos"
+    using valid_shift_aux unfolding shift_aux_def by auto
+  have I_ivl_w: "I = ivl w"
+    using valid_shift_aux by auto
+  define new_tstp where "new_tstp = (if left I = 0 then Inr tp else Inl (nt - (left I - 1)))"
+  have new_tstp_lt_isl: "tstp_lt new_tstp (nt - (left I - 1)) (tp + 1)"
+    "isl new_tstp \<longleftrightarrow> left I > 0"
+    by (auto simp add: new_tstp_def tstp_lt_def)
+  define tmp where "tmp = \<Union>((\<lambda>as. case Mapping.lookup a1_map (proj_tuple maskL as) of None \<Rightarrow>
+    (if \<not>pos then {(tp - len, as)} else {})
+    | Some tp' \<Rightarrow> if pos then {(max (tp - len) tp', as)}
+    else {(max (tp - len) (tp' + 1), as)}) ` rel2) \<union> (if left I = 0 then {tp} \<times> rel2 else {})"
+  have a1_map_lookup: "\<And>as tp'. Mapping.lookup a1_map as = Some tp' \<Longrightarrow> tp' < tp"
+    using valid_shift_aux(1) Mapping_keys_intro by force
+  then have fst_tmp: "\<And>tp'. tp' \<in> fst ` tmp \<Longrightarrow> tp - len \<le> tp' \<and> tp' < tp + 1"
+    unfolding tmp_def by (auto simp add: less_SucI split: option.splits if_splits)
+  have snd_tmp: "\<And>tp'. table n R (snd ` tmp)"
+    using tabs(2) unfolding tmp_def
+    by (auto simp add: table_def split: if_splits option.splits)
+  define a2_map' where "a2_map' = Mapping.update (tp + 1) Mapping.empty
+    (upd_nested a2_map new_tstp (max_tstp new_tstp) tmp)"
+  define a1_map' where "a1_map' = (if pos then Mapping.filter (\<lambda>as _. as \<in> rel1)
+    (upd_set a1_map (\<lambda>_. tp) (rel1 - Mapping.keys a1_map)) else upd_set a1_map (\<lambda>_. tp) rel1)"
+  define tss' where "tss' = append_queue nt tss"
+  have add_new_mmuaux_eq: "add_new_mmuaux rel1 rel2 nt aux = (tp + 1, len + 1, tss', I, pos,
+    maskL, maskR, a1_map', a2_map', done, done_length)"
+    using shift_aux_def new_tstp_def tmp_def a2_map'_def a1_map'_def tss'_def
+    by (auto simp only: add_new_mmuaux.simps Let_def)
+  have update_until_eq: "update_until I pos rel1 rel2 nt auxlist =
+    (map (\<lambda>x. case x of (t, a1, a2) \<Rightarrow> (t, if pos then join a1 True rel1 else a1 \<union> rel1,
+      if mem (nt - t) I then a2 \<union> join rel2 pos a1 else a2)) auxlist) @
+    [(nt, rel1, if left I = 0 then rel2 else empty_table)]"
+    unfolding update_until_def by simp
+  have len_done_auxlist: "length done \<le> length auxlist"
+    using valid_shift_aux by auto
+  have auxlist_split: "auxlist = take (length done) auxlist @ drop (length done) auxlist"
+    using len_done_auxlist by auto
+  have lin_tss': "linearize tss' = linearize tss @ [nt]"
+    unfolding tss'_def append_queue_rep by (rule refl)
+  have len_lin_tss': "length (linearize tss') = len + 1"
+    unfolding lin_tss' using valid_shift_aux by auto
+  have tmp: "sorted (linearize tss)" "\<And>t. t \<in> set (linearize tss) \<Longrightarrow> t \<le> current w"
+    using valid_shift_aux by auto
+  have sorted_lin_tss': "sorted (linearize tss')"
+    unfolding lin_tss' using tmp(1) le_trans[OF _ assms(4), OF tmp(2)]
+    by (simp add: sorted_append)
+  have in_lin_tss: "\<And>t. t \<in> set (linearize tss) \<Longrightarrow>
+    t \<le> current w \<and> enat (current w) \<le> enat t + right I"
+    using valid_shift_aux(1) by auto
+  then have set_lin_tss': "\<forall>t \<in> set (linearize tss'). t \<le> nt \<and> enat nt \<le> enat t + right I"
+    unfolding lin_tss' I_ivl_w using le_trans[OF _ assms(4)] valid_shift_aux(2)
+    by (auto simp add: not_less)
+  have a1_map'_keys: "Mapping.keys a1_map' \<subseteq> Mapping.keys a1_map \<union> rel1"
+    unfolding a1_map'_def using Mapping.keys_filter Mapping_upd_set_keys
+    by (auto simp add: Mapping_upd_set_keys split: if_splits dest: Mapping_keys_filterD)
+  then have tab_a1_map'_keys: "table n L (Mapping.keys a1_map')"
+    using valid_shift_aux(1) tabs(1) by (auto simp add: table_def)
+  have a2_map_keys: "Mapping.keys a2_map = {tp - len..tp}"
+    using valid_shift_aux by auto
+  have a2_map'_keys: "Mapping.keys a2_map' = {tp - len..tp + 1}"
+    unfolding a2_map'_def Mapping.keys_update upd_nested_keys a2_map_keys using fst_tmp
+    by fastforce
+  then have a2_map'_keys': "Mapping.keys a2_map' = {tp + 1 - (len + 1)..tp + 1}"
+    by auto
+  have len_upd_until: "length done + (len + 1) = length (update_until I pos rel1 rel2 nt auxlist)"
+    using valid_shift_aux unfolding update_until_eq by auto
+  have set_take_auxlist: "\<And>x. x \<in> set (take (length done) auxlist) \<Longrightarrow> check_before I nt x"
+    using valid_shift_aux by auto
+  have list_all2_triple: "list_all2 (\<lambda>x y. triple_eq_pair x y (\<lambda>tp'. filter_a1_map pos tp' a1_map)
+    (\<lambda>ts' tp'. filter_a2_map I ts' tp' a2_map)) (drop (length done) auxlist)
+    (zip (linearize tss) [tp - len..<tp])"
+    using valid_shift_aux by auto
+  have set_drop_auxlist: "\<And>x. x \<in> set (drop (length done) auxlist) \<Longrightarrow> \<not>check_before I nt x"
+    using valid_shift_aux(2)[OF list_all2_zip[OF list_all2_triple,
+      of "\<lambda>y. y \<in> set (linearize tss)"]]
+    unfolding I_ivl_w by auto
+  have length_done_auxlist: "length done \<le> length auxlist"
+    using valid_shift_aux by auto
+  have take_auxlist_takeWhile: "take (length done) auxlist = takeWhile (check_before I nt) auxlist"
+    using take_length_takeWhile[OF length_done_auxlist set_take_auxlist set_drop_auxlist] .
+  have set_take_auxlist': "\<And>x. x \<in> set (take (length done)
+    (update_until I pos rel1 rel2 nt auxlist)) \<Longrightarrow> check_before I nt x"
+    by (metis (no_types, lifting) add_right_cancel auxlist_split length_append length_done_auxlist
+        length_drop length_map map_proj_thd_update_until
+        ordered_cancel_comm_monoid_diff_class.add_diff_inverse set_takeWhileD
+        takeWhile_eq_take take_auxlist_takeWhile)
+  have rev_done: "rev done = map proj_thd (take (length done) auxlist)"
+    using valid_shift_aux by auto
+  moreover have "\<dots> = map proj_thd (takeWhile (check_before I nt)
+    (update_until I pos rel1 rel2 nt auxlist))"
+    by (simp add: take_auxlist_takeWhile map_proj_thd_update_until)
+  finally have rev_done': "rev done = map proj_thd (take (length done)
+    (update_until I pos rel1 rel2 nt auxlist))"
+    by (metis length_map length_rev takeWhile_eq_take)
+  have map_fst_auxlist_take: "\<And>t. t \<in> set (map fst (take (length done) auxlist)) \<Longrightarrow> t \<le> nt"
+    using set_take_auxlist
+    by auto (meson add_increasing2 enat_ord_simps(1) le_cases not_less zero_le)
+  have map_fst_auxlist_drop: "\<And>t. t \<in> set (map fst (drop (length done) auxlist)) \<Longrightarrow> t \<le> nt"
+    using in_lin_tss[OF list_all2_zip[OF list_all2_triple, of "\<lambda>y. y \<in> set (linearize tss)"]]
+      assms(4) dual_order.trans by auto blast
+  have set_drop_auxlist_cong: "\<And>x t a1 a2. x \<in> set (drop (length done) auxlist) \<Longrightarrow>
+    x = (t, a1, a2) \<Longrightarrow> mem (nt - t) I \<longleftrightarrow> left I \<le> nt - t"
+  proof -
+    fix x t a1 a2
+    assume "x \<in> set (drop (length done) auxlist)" "x = (t, a1, a2)"
+    then have "enat t + right I \<ge> enat nt"
+      using set_drop_auxlist not_less
+      by auto blast
+    then have "right I \<ge> enat (nt - t)"
+      apply (induction t arbitrary: nt)
+      using zero_enat_def apply auto
+      by (metis add_diff_cancel_left' diff_le_mono leD leI less_enat_iff plus_enat_simps(1))
+    then show "mem (nt - t) I \<longleftrightarrow> left I \<le> nt - t"
+      by auto
+  qed
+  have sorted_fst_auxlist: "sorted (map fst auxlist)"
+    using valid_shift_aux by auto
+  have set_map_fst_auxlist: "\<And>t. t \<in> set (map fst auxlist) \<Longrightarrow> t \<le> nt"
+    using arg_cong[OF auxlist_split, of "map fst", unfolded map_append]
+    apply (rule list_appendE)
+    using map_fst_auxlist_take map_fst_auxlist_drop by auto
+  have lookup_a1_map_keys: "\<And>xs tp'. Mapping.lookup a1_map xs = Some tp' \<Longrightarrow> tp' < tp"
+    using valid_shift_aux Mapping_keys_intro by force
+  have lookup_a1_map_keys': "\<forall>xs \<in> Mapping.keys a1_map'.
+    case Mapping.lookup a1_map' xs of Some tp' \<Rightarrow> tp' < tp + 1"
+    using lookup_a1_map_keys unfolding a1_map'_def
+    by (auto simp add: Mapping.lookup_filter Mapping_lookup_upd_set Mapping_upd_set_keys
+        split: option.splits dest: Mapping_keys_dest) fastforce+
+  have sorted_upd_until: "sorted (map fst (update_until I pos rel1 rel2 nt auxlist))"
+    using sorted_fst_auxlist set_map_fst_auxlist
+    unfolding update_until_eq
+    by (auto simp add: sorted_append comp_def fst_case)
+  have lookup_a2_map: "\<And>tp' m. Mapping.lookup a2_map tp' = Some m \<Longrightarrow>
+    table n R (Mapping.keys m) \<and> (\<forall>xs \<in> Mapping.keys m. case Mapping.lookup m xs of Some tstp \<Rightarrow>
+      tstp_lt tstp (current w - (left I - 1)) tp \<and> (isl tstp \<longleftrightarrow> left I > 0))"
+    using valid_shift_aux(1) Mapping_keys_intro by force
+  then have lookup_a2_map': "\<And>tp' m xs tstp. Mapping.lookup a2_map tp' = Some m \<Longrightarrow>
+    Mapping.lookup m xs = Some tstp \<Longrightarrow> tstp_lt tstp (nt - (left I - 1)) tp \<and>
+    isl tstp = (0 < left I)"
+    using Mapping_keys_intro assms(4) by (force simp add: tstp_lt_def split: sum.splits)
+  have lookup_a2_map'_keys: "\<forall>tp' \<in> Mapping.keys a2_map'.
+    case Mapping.lookup a2_map' tp' of Some m \<Rightarrow> table n R (Mapping.keys m) \<and>
+    (\<forall>xs \<in> Mapping.keys m. case Mapping.lookup m xs of Some tstp \<Rightarrow>
+    tstp_lt tstp (nt - (left I - 1)) (tp + 1) \<and> isl tstp = (0 < left I))"
+  proof (rule ballI)
+    fix tp'
+    assume tp'_assm: "tp' \<in> Mapping.keys a2_map'"
+    then obtain m' where m'_def: "Mapping.lookup a2_map' tp' = Some m'"
+      by (auto dest: Mapping_keys_dest)
+    have "table n R (Mapping.keys m') \<and>
+      (\<forall>xs \<in> Mapping.keys m'. case Mapping.lookup m' xs of Some tstp \<Rightarrow>
+      tstp_lt tstp (nt - (left I - 1)) (tp + 1) \<and> isl tstp = (0 < left I))"
+    proof (cases "tp' = tp + 1")
+      case True
+      show ?thesis
+        using m'_def unfolding a2_map'_def True Mapping.lookup_update
+        by (auto simp add: table_def)
+    next
+      case False
+      then have tp'_in: "tp' \<in> Mapping.keys a2_map"
+        using tp'_assm unfolding a2_map_keys a2_map'_keys by auto
+      then obtain m where m_def: "Mapping.lookup a2_map tp' = Some m"
+        by (auto dest: Mapping_keys_dest)
+      have m'_alt: "m' = upd_set' m new_tstp (max_tstp new_tstp) {b. (tp', b) \<in> tmp}"
+        using m_def m'_def unfolding a2_map'_def Mapping.lookup_update_neq[OF False[symmetric]]
+          upd_nested_lookup
+        by auto
+      have "table n R (Mapping.keys m')"
+        using lookup_a2_map[OF m_def] snd_tmp unfolding m'_alt upd_set'_keys
+        by (auto simp add: table_def)
+      moreover have "\<forall>xs \<in> Mapping.keys m'. case Mapping.lookup m' xs of Some tstp \<Rightarrow>
+        tstp_lt tstp (nt - (left I - 1)) (tp + 1) \<and> isl tstp = (0 < left I)"
+      proof (rule ballI)
+        fix xs
+        assume xs_assm: "xs \<in> Mapping.keys m'"
+        then obtain tstp where tstp_def: "Mapping.lookup m' xs = Some tstp"
+          by (auto dest: Mapping_keys_dest)
+        have "tstp_lt tstp (nt - (left I - 1)) (tp + 1) \<and> isl tstp = (0 < left I)"
+        proof (cases "Mapping.lookup m xs")
+          case None
+          then show ?thesis
+            using tstp_def[unfolded m'_alt upd_set'_lookup] new_tstp_lt_isl
+            by (auto split: if_splits)
+        next
+          case (Some tstp')
+          show ?thesis
+          proof (cases "xs \<in> {b. (tp', b) \<in> tmp}")
+            case True
+            then have tstp_eq: "tstp = max_tstp new_tstp tstp'"
+              using tstp_def[unfolded m'_alt upd_set'_lookup] Some
+              by auto
+            show ?thesis
+              apply (rule max_tstpE[of new_tstp tstp'])
+              using lookup_a2_map'[OF m_def Some] new_tstp_lt_isl unfolding tstp_eq
+              by (auto simp add: tstp_lt_def split: sum.splits)
+          next
+            case False
+            then show ?thesis
+              using tstp_def[unfolded m'_alt upd_set'_lookup] lookup_a2_map'[OF m_def Some] Some
+              by (auto simp add: tstp_lt_def split: sum.splits)
+          qed
+        qed
+        then show "case Mapping.lookup m' xs of Some tstp \<Rightarrow>
+          tstp_lt tstp (nt - (left I - 1)) (tp + 1) \<and> isl tstp = (0 < left I)"
+          using tstp_def by auto
+      qed
+      ultimately show ?thesis
+        by auto
+    qed
+    then show "case Mapping.lookup a2_map' tp' of Some m \<Rightarrow> table n R (Mapping.keys m) \<and>
+      (\<forall>xs \<in> Mapping.keys m. case Mapping.lookup m xs of Some tstp \<Rightarrow>
+      tstp_lt tstp (nt - (left I - 1)) (tp + 1) \<and> isl tstp = (0 < left I))"
+      using m'_def by auto
+  qed
+  have tp_upt_Suc: "[tp + 1 - (len + 1)..<tp + 1] = [tp - len..<tp] @ [tp]"
+    using upt_Suc by auto
+  have map_eq: "map (\<lambda>x. case x of (t, a1, a2) \<Rightarrow> (t, if pos then join a1 True rel1 else a1 \<union> rel1,
+      if mem (nt - t) I then a2 \<union> join rel2 pos a1 else a2)) (drop (length done) auxlist) =
+    map (\<lambda>x. case x of (t, a1, a2) \<Rightarrow> (t, if pos then join a1 True rel1 else a1 \<union> rel1,
+      if left I \<le> nt - t then a2 \<union> join rel2 pos a1 else a2)) (drop (length done) auxlist)"
+    using set_drop_auxlist_cong by auto
+  have "drop (length done) (update_until I pos rel1 rel2 nt auxlist) =
+    map (\<lambda>x. case x of (t, a1, a2) \<Rightarrow> (t, if pos then join a1 True rel1 else a1 \<union> rel1,
+      if mem (nt - t) I then a2 \<union> join rel2 pos a1 else a2)) (drop (length done) auxlist) @
+    [(nt, rel1, if left I = 0 then rel2 else empty_table)]"
+    unfolding update_until_eq using len_done_auxlist drop_map by auto
+  note drop_update_until = this[unfolded map_eq]
+  have list_all2_old: "list_all2 (\<lambda>x y. triple_eq_pair x y (\<lambda>tp'. filter_a1_map pos tp' a1_map')
+    (\<lambda>ts' tp'. filter_a2_map I ts' tp' a2_map'))
+    (map (\<lambda>(t, a1, a2). (t, if pos then join a1 True rel1 else a1 \<union> rel1,
+      if left I \<le> nt - t then a2 \<union> join rel2 pos a1 else a2)) (drop (length done) auxlist))
+    (zip (linearize tss) [tp - len..<tp])"
+    unfolding list_all2_map1
+    using list_all2_triple
+  proof (rule list.rel_mono_strong)
+    fix tri pair
+    assume tri_pair_in: "tri \<in> set (drop (length done) auxlist)"
+      "pair \<in> set (zip (linearize tss) [tp - len..<tp])"
+    obtain t a1 a2 where tri_def: "tri = (t, a1, a2)"
+      by (cases tri) auto
+    obtain ts' tp' where pair_def: "pair = (ts', tp')"
+      by (cases pair) auto
+    assume "triple_eq_pair tri pair (\<lambda>tp'. filter_a1_map pos tp' a1_map)
+      (\<lambda>ts' tp'. filter_a2_map I ts' tp' a2_map)"
+    then have eqs: "t = ts'" "a1 = filter_a1_map pos tp' a1_map"
+      "a2 = filter_a2_map I ts' tp' a2_map"
+      unfolding tri_def pair_def by auto
+    have tp'_ge: "tp' \<ge> tp - len"
+      using tri_pair_in(2) unfolding pair_def
+      by (auto elim: in_set_zipE)
+    have tp'_lt_tp: "tp' < tp"
+      using tri_pair_in(2) unfolding pair_def
+      by (auto elim: in_set_zipE)
+    have ts'_in_lin_tss: "ts' \<in> set (linearize tss)"
+      using tri_pair_in(2) unfolding pair_def
+      by (auto elim: in_set_zipE)
+    then have ts'_nt: "ts' \<le> nt"
+      using valid_shift_aux(1) assms(4) by auto
+    then have t_nt: "t \<le> nt"
+      unfolding eqs(1) .
+    have "table n L (Mapping.keys a1_map)"
+      using valid_shift_aux by auto
+    then have a1_tab: "table n L a1"
+      unfolding eqs(2) filter_a1_map_def by (auto simp add: table_def)
+    have join_rel2_assms: "L \<subseteq> R" "maskL = join_mask n L"
+      using valid_shift_aux by auto
+    have join_rel2_eq: "join rel2 pos a1 = {xs \<in> rel2. proj_tuple_in_join pos maskL xs a1}"
+      using join_sub[OF join_rel2_assms(1) a1_tab tabs(2)] join_rel2_assms(2) by auto
+    have filter_sub_a2: "\<And>xs m' tp'' tstp. tp'' \<le> tp' \<Longrightarrow>
+      Mapping.lookup a2_map' tp'' = Some m' \<Longrightarrow> Mapping.lookup m' xs = Some tstp \<Longrightarrow>
+      ts_tp_lt' ts' tp' tstp \<Longrightarrow> (tstp = new_tstp \<Longrightarrow> False) \<Longrightarrow>
+      xs \<in> filter_a2_map I ts' tp' a2_map' \<Longrightarrow> xs \<in> a2"
+    proof -
+      fix xs m' tp'' tstp
+      assume m'_def: "tp'' \<le> tp'" "Mapping.lookup a2_map' tp'' = Some m'"
+        "Mapping.lookup m' xs = Some tstp" "ts_tp_lt' ts' tp' tstp"
+      have tp''_neq: "tp + 1 \<noteq> tp''"
+        using le_less_trans[OF m'_def(1) tp'_lt_tp] by auto
+      assume new_tstp_False: "tstp = new_tstp \<Longrightarrow> False"
+      show "xs \<in> a2"
+      proof (cases "Mapping.lookup a2_map tp''")
+        case None
+        then have m'_alt: "m' = upd_set' Mapping.empty new_tstp (max_tstp new_tstp)
+          {b. (tp'', b) \<in> tmp}"
+          using m'_def(2)[unfolded a2_map'_def Mapping.lookup_update_neq[OF tp''_neq]
+            upd_nested_lookup] by (auto split: option.splits if_splits)
+        then show ?thesis
+          using new_tstp_False m'_def(3)[unfolded m'_alt upd_set'_lookup Mapping.lookup_empty]
+          by (auto split: if_splits)
+      next
+        case (Some m)
+        then have m'_alt: "m' = upd_set' m new_tstp (max_tstp new_tstp) {b. (tp'', b) \<in> tmp}"
+          using m'_def(2)[unfolded a2_map'_def Mapping.lookup_update_neq[OF tp''_neq]
+            upd_nested_lookup] by (auto split: option.splits if_splits)
+        note lookup_m = Some
+        show ?thesis
+        proof (cases "Mapping.lookup m xs")
+          case None
+          then show ?thesis
+            using new_tstp_False m'_def(3)[unfolded m'_alt upd_set'_lookup]
+            by (auto split: if_splits)
+        next
+          case (Some tstp')
+          have tstp_ok: "tstp = tstp' \<Longrightarrow> xs \<in> a2"
+            using eqs(3) lookup_m Some m'_def unfolding filter_a2_map_def by auto
+          show ?thesis
+          proof (cases "xs \<in> {b. (tp'', b) \<in> tmp}")
+            case True
+            then have tstp_eq: "tstp = max_tstp new_tstp tstp'"
+              using m'_def(3)[unfolded m'_alt upd_set'_lookup Some] by auto
+            show ?thesis
+              apply (rule max_tstpE[of new_tstp tstp'])
+              using lookup_a2_map'[OF lookup_m Some] new_tstp_lt_isl(2)
+                tstp_eq new_tstp_False tstp_ok by auto
+          next
+            case False
+            then have "tstp = tstp'"
+              using m'_def(3)[unfolded m'_alt upd_set'_lookup Some] by auto
+            then show ?thesis
+              using tstp_ok by auto
+          qed
+        qed
+      qed
+    qed
+    have a2_sub_filter: "a2 \<subseteq> filter_a2_map I ts' tp' a2_map'"
+    proof (rule subsetI)
+      fix xs
+      assume xs_in: "xs \<in> a2"
+      then obtain tp'' m tstp where m_def: "tp'' \<le> tp'" "Mapping.lookup a2_map tp'' = Some m"
+        "Mapping.lookup m xs = Some tstp" "ts_tp_lt' ts' tp' tstp"
+        using eqs(3)[unfolded filter_a2_map_def] by (auto split: option.splits)
+      have tp''_in: "tp'' \<in> {tp - len..tp}"
+        using m_def(2) a2_map_keys by (auto intro!: Mapping_keys_intro)
+      then obtain m' where m'_def: "Mapping.lookup a2_map' tp'' = Some m'"
+        using a2_map'_keys
+        by (metis Mapping_keys_dest One_nat_def add_Suc_right add_diff_cancel_right'
+            atLeastatMost_subset_iff diff_zero le_eq_less_or_eq le_less_Suc_eq subsetD)
+      have tp''_neq: "tp + 1 \<noteq> tp''"
+        using m_def(1) tp'_lt_tp by auto
+      have m'_alt: "m' = upd_set' m new_tstp (max_tstp new_tstp) {b. (tp'', b) \<in> tmp}"
+        using m'_def[unfolded a2_map'_def Mapping.lookup_update_neq[OF tp''_neq] m_def(2)
+          upd_nested_lookup] by (auto split: option.splits if_splits)
+      show "xs \<in> filter_a2_map I ts' tp' a2_map'"
+      proof (cases "xs \<in> {b. (tp'', b) \<in> tmp}")
+        case True
+        then have "Mapping.lookup m' xs = Some (max_tstp new_tstp tstp)"
+          unfolding m'_alt upd_set'_lookup m_def(3) by auto
+        moreover have "ts_tp_lt' ts' tp' (max_tstp new_tstp tstp)"
+          apply (rule max_tstp_intro''''[OF _ m_def(4)])
+          using new_tstp_lt_isl(2) lookup_a2_map'[OF m_def(2,3)] by auto
+        ultimately show ?thesis
+          unfolding filter_a2_map_def using m_def(1) m'_def m_def(4) by auto
+      next
+        case False
+        then have "Mapping.lookup m' xs = Some tstp"
+          unfolding m'_alt upd_set'_lookup m_def(3) by auto
+        then show ?thesis
+          unfolding filter_a2_map_def using m_def(1) m'_def m_def by auto
+      qed
+    qed
+    have "pos \<Longrightarrow> filter_a1_map pos tp' a1_map' = join a1 True rel1"
+    proof -
+      assume pos: pos
+      have join_eq: "join a1 True rel1 = a1 \<inter> rel1"
+        using join_eq[OF tabs(1) a1_tab] by auto
+      show "filter_a1_map pos tp' a1_map' = join a1 True rel1"
+        using eqs(2) pos tp'_lt_tp unfolding filter_a1_map_def a1_map'_def join_eq
+        apply (auto simp add: Mapping.lookup_filter Mapping_lookup_upd_set
+            intro: Mapping_keys_intro dest: Mapping_keys_dest split: if_splits option.splits)
+        using Mapping_keys_filterD by fastforce+
+    qed
+    moreover have "\<not>pos \<Longrightarrow> filter_a1_map pos tp' a1_map' = a1 \<union> rel1"
+      using eqs(2) tp'_lt_tp unfolding filter_a1_map_def a1_map'_def
+      by (auto simp add: Mapping.lookup_filter Mapping_lookup_upd_set intro: Mapping_keys_intro
+          dest: Mapping_keys_filterD Mapping_keys_dest split: option.splits)
+    moreover have "left I \<le> nt - t \<Longrightarrow> filter_a2_map I ts' tp' a2_map' = a2 \<union> join rel2 pos a1"
+    proof (rule set_eqI, rule iffI)
+      fix xs
+      assume in_int: "left I \<le> nt - t"
+      assume xs_in: "xs \<in> filter_a2_map I ts' tp' a2_map'"
+      then obtain m' tp'' tstp where m'_def: "tp'' \<le> tp'" "Mapping.lookup a2_map' tp'' = Some m'"
+        "Mapping.lookup m' xs = Some tstp" "ts_tp_lt' ts' tp' tstp"
+        unfolding filter_a2_map_def by (fastforce split: option.splits)
+      show "xs \<in> a2 \<union> join rel2 pos a1"
+      proof (cases "tstp = new_tstp")
+        case True
+        note tstp_new_tstp = True
+        have tp''_neq: "tp + 1 \<noteq> tp''"
+          using m'_def(1) tp'_lt_tp by auto
+        have tp''_in: "tp'' \<in> {tp - len..tp}"
+          using m'_def(1,2) tp'_lt_tp a2_map'_keys
+          by (auto intro!: Mapping_keys_intro)
+        obtain m where m_def: "Mapping.lookup a2_map tp'' = Some m"
+          "m' = upd_set' m new_tstp (max_tstp new_tstp) {b. (tp'', b) \<in> tmp}"
+          using m'_def(2)[unfolded a2_map'_def Mapping.lookup_update_neq[OF tp''_neq]
+            upd_nested_lookup] tp''_in a2_map_keys
+          by (fastforce dest: Mapping_keys_dest split: option.splits if_splits)
+        show ?thesis
+        proof (cases "Mapping.lookup m xs = Some new_tstp")
+          case True
+          then show ?thesis
+            using eqs(3) m'_def(1) m_def(1) m'_def tstp_new_tstp
+            unfolding filter_a2_map_def by auto
+        next
+          case False
+          then have xs_in_snd_tmp: "xs \<in> {b. (tp'', b) \<in> tmp}"
+            using m'_def(3)[unfolded m_def(2) upd_set'_lookup True]
+            by (auto split: if_splits)
+          then have xs_in_rel2: "xs \<in> rel2"
+            unfolding tmp_def
+            by (auto split: if_splits option.splits)
+          show ?thesis
+          proof (cases pos)
+            case True
+            obtain tp''' where tp'''_def: "Mapping.lookup a1_map (proj_tuple maskL xs) = Some tp'''"
+              "if pos then tp'' = max (tp - len) tp''' else tp'' = max (tp - len) (tp''' + 1)"
+              using xs_in_snd_tmp m'_def(1) tp'_lt_tp True
+              unfolding tmp_def by (auto split: option.splits if_splits)
+            have "proj_tuple maskL xs \<in> a1"
+              using eqs(2)[unfolded filter_a1_map_def] True m'_def(1) tp'''_def
+              by (auto intro: Mapping_keys_intro)
+            then show ?thesis
+              using True xs_in_rel2 unfolding proj_tuple_in_join_def join_rel2_eq by auto
+          next
+            case False
+            show ?thesis
+            proof (cases "Mapping.lookup a1_map (proj_tuple maskL xs)")
+              case None
+              then show ?thesis
+                using xs_in_rel2 False eqs(2)[unfolded filter_a1_map_def]
+                unfolding proj_tuple_in_join_def join_rel2_eq
+                by (auto dest: Mapping_keys_dest)
+            next
+              case (Some tp''')
+              then have "tp'' = max (tp - len) (tp''' + 1)"
+                using xs_in_snd_tmp m'_def(1) tp'_lt_tp False
+                unfolding tmp_def by (auto split: option.splits if_splits)
+              then have "tp''' < tp'"
+                using m'_def(1) by auto
+              then have "proj_tuple maskL xs \<notin> a1"
+                using eqs(2)[unfolded filter_a1_map_def] True m'_def(1) Some False
+                by (auto intro: Mapping_keys_intro)
+              then show ?thesis
+                using xs_in_rel2 False unfolding proj_tuple_in_join_def join_rel2_eq by auto
+            qed
+          qed
+        qed
+      next
+        case False
+        then show ?thesis
+          using filter_sub_a2[OF m'_def _ xs_in] by auto
+      qed
+    next
+      fix xs
+      assume in_int: "left I \<le> nt - t"
+      assume xs_in: "xs \<in> a2 \<union> join rel2 pos a1"
+      then have "xs \<in> a2 \<union> (join rel2 pos a1 - a2)"
+        by auto
+      then show "xs \<in> filter_a2_map I ts' tp' a2_map'"
+      proof (rule UnE)
+        assume "xs \<in> a2"
+        then show "xs \<in> filter_a2_map I ts' tp' a2_map'"
+          using a2_sub_filter by auto
+      next
+        assume "xs \<in> join rel2 pos a1 - a2"
+        then have xs_props: "xs \<in> rel2" "xs \<notin> a2" "proj_tuple_in_join pos maskL xs a1"
+          unfolding join_rel2_eq by auto
+        have ts_tp_lt'_new_tstp: "ts_tp_lt' ts' tp' new_tstp"
+          using tp'_lt_tp in_int t_nt eqs(1) unfolding new_tstp_def
+          by (auto simp add: ts_tp_lt'_def)
+        show "xs \<in> filter_a2_map I ts' tp' a2_map'"
+        proof (cases pos)
+          case True
+          then obtain tp''' where tp'''_def: "tp''' \<le> tp'"
+            "Mapping.lookup a1_map (proj_tuple maskL xs) = Some tp'''"
+            using eqs(2)[unfolded filter_a1_map_def] xs_props(3)[unfolded proj_tuple_in_join_def]
+            by (auto dest: Mapping_keys_dest)
+          define wtp where "wtp \<equiv> max (tp - len) tp'''"
+          have wtp_xs_in: "(wtp, xs) \<in> tmp"
+            unfolding wtp_def using tp'''_def tmp_def xs_props(1) True by fastforce
+          have wtp_le: "wtp \<le> tp'"
+            using tp'''_def(1) tp'_ge unfolding wtp_def by auto
+          have wtp_in: "wtp \<in> {tp - len..tp}"
+            using tp'''_def(1) tp'_lt_tp unfolding wtp_def by auto
+          have wtp_neq: "tp + 1 \<noteq> wtp"
+            using wtp_in by auto
+          obtain m where m_def: "Mapping.lookup a2_map wtp = Some m"
+            using wtp_in a2_map_keys Mapping_keys_dest by fastforce
+          obtain m' where m'_def: "Mapping.lookup a2_map' wtp = Some m'"
+            using wtp_in a2_map'_keys Mapping_keys_dest by fastforce
+          have m'_alt: "m' = upd_set' m new_tstp (max_tstp new_tstp) {b. (wtp, b) \<in> tmp}"
+            using m'_def[unfolded a2_map'_def Mapping.lookup_update_neq[OF wtp_neq]
+              upd_nested_lookup m_def] by auto
+          show ?thesis
+          proof (cases "Mapping.lookup m xs")
+            case None
+            have "Mapping.lookup m' xs = Some new_tstp"
+              using wtp_xs_in unfolding m'_alt upd_set'_lookup None by auto
+            then show ?thesis
+              unfolding filter_a2_map_def using wtp_le m'_def ts_tp_lt'_new_tstp by auto
+          next
+            case (Some tstp')
+            have "Mapping.lookup m' xs = Some (max_tstp new_tstp tstp')"
+              using wtp_xs_in unfolding m'_alt upd_set'_lookup Some by auto
+            moreover have "ts_tp_lt' ts' tp' (max_tstp new_tstp tstp')"
+              apply (rule max_tstp_intro''')
+              using ts_tp_lt'_new_tstp lookup_a2_map'[OF m_def Some] new_tstp_lt_isl
+              by auto
+            ultimately show ?thesis
+              using lookup_a2_map'[OF m_def Some] wtp_le m'_def
+              unfolding filter_a2_map_def by auto
+          qed
+        next
+          case False
+          show ?thesis
+          proof (cases "Mapping.lookup a1_map (proj_tuple maskL xs)")
+            case None
+            then have in_tmp: "(tp - len, xs) \<in> tmp" 
+              using tmp_def False xs_props(1) by fastforce
+            obtain m where m_def: "Mapping.lookup a2_map (tp - len) = Some m"
+              using a2_map_keys by (fastforce dest: Mapping_keys_dest)
+            obtain m' where m'_def: "Mapping.lookup a2_map' (tp - len) = Some m'"
+              using a2_map'_keys by (fastforce dest: Mapping_keys_dest)
+            have tp_neq: "tp + 1 \<noteq> tp - len"
+              by auto
+            have m'_alt: "m' = upd_set' m new_tstp (max_tstp new_tstp) {b. (tp - len, b) \<in> tmp}"
+              using m'_def[unfolded a2_map'_def Mapping.lookup_update_neq[OF tp_neq]
+                upd_nested_lookup m_def] by auto
+            show ?thesis
+            proof (cases "Mapping.lookup m xs")
+              case None
+              have "Mapping.lookup m' xs = Some new_tstp"
+                unfolding m'_alt upd_set'_lookup None using in_tmp by auto
+              then show ?thesis
+                unfolding filter_a2_map_def using tp'_ge m'_def ts_tp_lt'_new_tstp by auto
+            next
+              case (Some tstp')
+              have "Mapping.lookup m' xs = Some (max_tstp new_tstp tstp')"
+                unfolding m'_alt upd_set'_lookup Some using in_tmp by auto
+              moreover have "ts_tp_lt' ts' tp' (max_tstp new_tstp tstp')"
+                apply (rule max_tstp_intro''')
+                using ts_tp_lt'_new_tstp lookup_a2_map'[OF m_def Some] new_tstp_lt_isl
+                by auto
+              ultimately show ?thesis
+                unfolding filter_a2_map_def using tp'_ge m'_def by auto
+            qed
+          next
+            case (Some tp''')
+            then have tp'_gt: "tp' > tp'''"
+              using xs_props(3)[unfolded proj_tuple_in_join_def] eqs(2)[unfolded filter_a1_map_def]
+                False by (auto intro: Mapping_keys_intro)
+            define wtp where "wtp \<equiv> max (tp - len) (tp''' + 1)"
+            have wtp_xs_in: "(wtp, xs) \<in> tmp"
+              unfolding wtp_def tmp_def using xs_props(1) Some False by fastforce
+            have wtp_le: "wtp \<le> tp'"
+              using tp'_ge tp'_gt unfolding wtp_def by auto
+            have wtp_in: "wtp \<in> {tp - len..tp}"
+              using tp'_lt_tp tp'_gt unfolding wtp_def by auto
+            have wtp_neq: "tp + 1 \<noteq> wtp"
+              using wtp_in by auto
+            obtain m where m_def: "Mapping.lookup a2_map wtp = Some m"
+              using wtp_in a2_map_keys Mapping_keys_dest by fastforce
+            obtain m' where m'_def: "Mapping.lookup a2_map' wtp = Some m'"
+              using wtp_in a2_map'_keys Mapping_keys_dest by fastforce
+            have m'_alt: "m' = upd_set' m new_tstp (max_tstp new_tstp) {b. (wtp, b) \<in> tmp}"
+              using m'_def[unfolded a2_map'_def Mapping.lookup_update_neq[OF wtp_neq]
+                upd_nested_lookup m_def] by auto
+            show ?thesis
+            proof (cases "Mapping.lookup m xs")
+              case None
+              have "Mapping.lookup m' xs = Some new_tstp"
+                using wtp_xs_in unfolding m'_alt upd_set'_lookup None by auto
+              then show ?thesis
+                unfolding filter_a2_map_def using wtp_le m'_def ts_tp_lt'_new_tstp by auto
+            next
+              case (Some tstp')
+              have "Mapping.lookup m' xs = Some (max_tstp new_tstp tstp')"
+                using wtp_xs_in unfolding m'_alt upd_set'_lookup Some by auto
+              moreover have "ts_tp_lt' ts' tp' (max_tstp new_tstp tstp')"
+                apply (rule max_tstp_intro''')
+                using ts_tp_lt'_new_tstp lookup_a2_map'[OF m_def Some] new_tstp_lt_isl
+                by auto
+              ultimately show ?thesis
+                using lookup_a2_map'[OF m_def Some] wtp_le m'_def
+                unfolding filter_a2_map_def by auto
+            qed
+          qed
+        qed
+      qed
+    qed
+    moreover have "nt - t < left I \<Longrightarrow> filter_a2_map I ts' tp' a2_map' = a2"
+    proof (rule set_eqI, rule iffI)
+      fix xs
+      assume out: "nt - t < left I"
+      assume xs_in: "xs \<in> filter_a2_map I ts' tp' a2_map'"
+      then obtain m' tp'' tstp where m'_def: "tp'' \<le> tp'" "Mapping.lookup a2_map' tp'' = Some m'"
+        "Mapping.lookup m' xs = Some tstp" "ts_tp_lt' ts' tp' tstp"
+        unfolding filter_a2_map_def by (fastforce split: option.splits)
+      have new_tstp_False: "tstp = new_tstp \<Longrightarrow> False"
+        using m'_def t_nt out tp'_lt_tp unfolding eqs(1)
+        by (auto simp add: ts_tp_lt'_def new_tstp_def)
+      show "xs \<in> a2"
+        using filter_sub_a2[OF m'_def new_tstp_False xs_in] .
+    next
+      fix xs
+      assume "xs \<in> a2"
+      then show "xs \<in> filter_a2_map I ts' tp' a2_map'"
+        using a2_sub_filter by auto
+    qed
+    ultimately show "triple_eq_pair (case tri of (t, a1, a2) \<Rightarrow>
+      (t, if pos then join a1 True rel1 else a1 \<union> rel1,
+      if left I \<le> nt - t then a2 \<union> join rel2 pos a1 else a2))
+      pair (\<lambda>tp'. filter_a1_map pos tp' a1_map') (\<lambda>ts' tp'. filter_a2_map I ts' tp' a2_map')"
+      using eqs unfolding tri_def pair_def by auto
+  qed
+  have filter_a1_map_rel1: "filter_a1_map pos tp a1_map' = rel1"
+    unfolding filter_a1_map_def a1_map'_def
+    apply (auto simp add: a1_map_lookup less_imp_le_nat Mapping.lookup_filter
+        Mapping_lookup_upd_set keys_is_none_rep dest: Mapping_keys_filterD
+        intro: Mapping_keys_intro split: option.splits)
+    using leD lookup_a1_map_keys by auto
+  have filter_a1_map_rel2: "filter_a2_map I nt tp a2_map' =
+    (if left I = 0 then rel2 else empty_table)"
+  proof (cases "left I = 0")
+    case True
+    note left_I_zero = True
+    have "\<And>tp' m' xs tstp. tp' \<le> tp \<Longrightarrow> Mapping.lookup a2_map' tp' = Some m' \<Longrightarrow>
+      Mapping.lookup m' xs = Some tstp \<Longrightarrow> ts_tp_lt' nt tp tstp \<Longrightarrow> xs \<in> rel2"
+    proof -
+      fix tp' m' xs tstp
+      assume lassms: "tp' \<le> tp" "Mapping.lookup a2_map' tp' = Some m'"
+        "Mapping.lookup m' xs = Some tstp" "ts_tp_lt' nt tp tstp"
+      have tp'_neq: "tp + 1 \<noteq> tp'"
+        using lassms(1) by auto
+      have tp'_in: "tp' \<in> {tp - len..tp}"
+        using lassms(1,2) a2_map'_keys tp'_neq by (auto intro!: Mapping_keys_intro)
+      obtain m where m_def: "Mapping.lookup a2_map tp' = Some m"
+        "m' = upd_set' m new_tstp (max_tstp new_tstp) {b. (tp', b) \<in> tmp}"
+        using lassms(2)[unfolded a2_map'_def Mapping.lookup_update_neq[OF tp'_neq]
+          upd_nested_lookup] tp'_in a2_map_keys
+        by (fastforce dest: Mapping_keys_dest intro: Mapping_keys_intro split: option.splits)
+      have "xs \<in> {b. (tp', b) \<in> tmp}"
+      proof (rule ccontr)
+        assume "xs \<notin> {b. (tp', b) \<in> tmp}"
+        then have Some: "Mapping.lookup m xs = Some tstp"
+          using lassms(3)[unfolded m_def(2) upd_set'_lookup] by auto
+        show "False"
+          using lookup_a2_map'[OF m_def(1) Some] lassms(4)
+          by (auto simp add: tstp_lt_def ts_tp_lt'_def split: sum.splits)
+      qed
+      then show "xs \<in> rel2"
+        unfolding tmp_def by (auto split: option.splits if_splits)
+    qed
+    moreover have "\<And>xs. xs \<in> rel2 \<Longrightarrow> \<exists>m' tstp. Mapping.lookup a2_map' tp = Some m' \<and>
+      Mapping.lookup m' xs = Some tstp \<and> ts_tp_lt' nt tp tstp"
+    proof -
+      fix xs
+      assume lassms: "xs \<in> rel2"
+      obtain m' where m'_def: "Mapping.lookup a2_map' tp = Some m'"
+        using a2_map'_keys by (fastforce dest: Mapping_keys_dest)
+      have tp_neq: "tp + 1 \<noteq> tp"
+        by auto
+      obtain m where m_def: "Mapping.lookup a2_map tp = Some m"
+        "m' = upd_set' m new_tstp (max_tstp new_tstp) {b. (tp, b) \<in> tmp}"
+        using m'_def a2_map_keys unfolding a2_map'_def Mapping.lookup_update_neq[OF tp_neq]
+          upd_nested_lookup
+        by (auto dest: Mapping_keys_dest split: option.splits if_splits)
+           (metis Mapping_keys_dest atLeastAtMost_iff diff_le_self le_eq_less_or_eq
+            option.simps(3))
+      have xs_in_tmp: "xs \<in> {b. (tp, b) \<in> tmp}"
+        using lassms left_I_zero unfolding tmp_def by auto
+      show "\<exists>m' tstp. Mapping.lookup a2_map' tp = Some m' \<and>
+        Mapping.lookup m' xs = Some tstp \<and> ts_tp_lt' nt tp tstp"
+      proof (cases "Mapping.lookup m xs")
+        case None
+        moreover have "Mapping.lookup m' xs = Some new_tstp"
+          using xs_in_tmp unfolding m_def(2) upd_set'_lookup None by auto
+        moreover have "ts_tp_lt' nt tp new_tstp"
+          using left_I_zero new_tstp_def by (auto simp add: ts_tp_lt'_def)
+        ultimately show ?thesis
+          using xs_in_tmp m_def
+          unfolding a2_map'_def Mapping.lookup_update_neq[OF tp_neq] upd_nested_lookup by auto
+      next
+        case (Some tstp')
+        moreover have "Mapping.lookup m' xs = Some (max_tstp new_tstp tstp')"
+          using xs_in_tmp unfolding m_def(2) upd_set'_lookup Some by auto
+        moreover have "ts_tp_lt' nt tp (max_tstp new_tstp tstp')"
+          apply (rule max_tstpE[of new_tstp tstp'])
+          using lookup_a2_map'[OF m_def(1) Some] new_tstp_lt_isl left_I_zero
+          by (auto simp add: sum.discI(1) new_tstp_def ts_tp_lt'_def tstp_lt_def split: sum.splits)
+        ultimately show ?thesis
+          using xs_in_tmp m_def
+          unfolding a2_map'_def Mapping.lookup_update_neq[OF tp_neq] upd_nested_lookup by auto
+      qed
+    qed
+    ultimately show ?thesis
+      using True by (fastforce simp add: filter_a2_map_def split: option.splits)
+  next
+    case False
+    note left_I_pos = False
+    have "\<And>tp' m xs tstp. tp' \<le> tp \<Longrightarrow> Mapping.lookup a2_map' tp' = Some m \<Longrightarrow>
+      Mapping.lookup m xs = Some tstp \<Longrightarrow> \<not>(ts_tp_lt' nt tp tstp)"
+    proof -
+      fix tp' m' xs tstp
+      assume lassms: "tp' \<le> tp" "Mapping.lookup a2_map' tp' = Some m'"
+        "Mapping.lookup m' xs = Some tstp"
+      from lassms(1) have tp'_neq_Suc_tp: "tp + 1 \<noteq> tp'"
+        by auto
+      show "\<not>(ts_tp_lt' nt tp tstp)"
+      proof (cases "Mapping.lookup a2_map tp'")
+        case None
+        then have tp'_in_tmp: "tp' \<in> fst ` tmp" and
+          m'_alt: "m' = upd_set' Mapping.empty new_tstp (max_tstp new_tstp) {b. (tp', b) \<in> tmp}"
+          using lassms(2) unfolding a2_map'_def Mapping.lookup_update_neq[OF tp'_neq_Suc_tp]
+            upd_nested_lookup by (auto split: if_splits)
+        then have "tstp = new_tstp"
+          using lassms(3)[unfolded m'_alt upd_set'_lookup]
+          by (auto simp add: Mapping.lookup_empty split: if_splits)
+        then show ?thesis
+          using False by (auto simp add: ts_tp_lt'_def new_tstp_def split: if_splits sum.splits)
+      next
+        case (Some m)
+        then have m'_alt: "m' = upd_set' m new_tstp (max_tstp new_tstp) {b. (tp', b) \<in> tmp}"
+          using lassms(2) unfolding a2_map'_def Mapping.lookup_update_neq[OF tp'_neq_Suc_tp]
+            upd_nested_lookup by auto
+        note lookup_a2_map_tp' = Some
+        show ?thesis
+        proof (cases "Mapping.lookup m xs")
+          case None
+          then have "tstp = new_tstp"
+            using lassms(3) unfolding m'_alt upd_set'_lookup by (auto split: if_splits)
+          then show ?thesis
+            using False by (auto simp add: ts_tp_lt'_def new_tstp_def split: if_splits sum.splits)
+        next
+          case (Some tstp')
+          show ?thesis
+          proof (cases "xs \<in> {b. (tp', b) \<in> tmp}")
+            case True
+            then have tstp_eq: "tstp = max_tstp new_tstp tstp'"
+              using lassms(3)
+              unfolding m'_alt upd_set'_lookup Some by auto
+            show ?thesis
+              apply (rule max_tstpE[of new_tstp tstp'])
+              using lookup_a2_map'[OF lookup_a2_map_tp' Some] new_tstp_lt_isl left_I_pos
+              by (auto simp add: tstp_eq tstp_lt_def ts_tp_lt'_def split: sum.splits)
+          next
+            case False
+            then show ?thesis
+              using lassms(3) lookup_a2_map'[OF lookup_a2_map_tp' Some]
+              unfolding m'_alt upd_set'_lookup Some
+              by (auto simp add: ts_tp_lt'_def tstp_lt_def split: sum.splits)
+          qed
+        qed
+      qed
+    qed
+    then show ?thesis
+      using False by (auto simp add: filter_a2_map_def empty_table_def split: option.splits)
+  qed
+  have zip_dist: "zip (linearize tss @ [nt]) ([tp - len..<tp] @ [tp]) =
+    zip (linearize tss) [tp - len..<tp] @ [(nt, tp)]"
+    using valid_shift_aux(1) by auto
+  have list_all2': "list_all2 (\<lambda>x y. triple_eq_pair x y (\<lambda>tp'. filter_a1_map pos tp' a1_map')
+    (\<lambda>ts' tp'. filter_a2_map I ts' tp' a2_map'))
+    (drop (length done) (update_until I pos rel1 rel2 nt auxlist))
+    (zip (linearize tss') [tp + 1 - (len + 1)..<tp + 1])"
+    unfolding lin_tss' tp_upt_Suc drop_update_until zip_dist
+    using filter_a1_map_rel1 filter_a1_map_rel2 list_all2_appendI[OF list_all2_old]
+    by auto
+  have cur_w': "current w' = nt"
+    using assms(5) by auto
+  have ivl_w': "ivl w' = I"
+    using assms(5) I_ivl_w by auto
+  show ?thesis
+    using valid_shift_aux len_lin_tss' sorted_lin_tss' set_lin_tss' tab_a1_map'_keys a2_map'_keys'
+      len_upd_until sorted_upd_until lookup_a1_map_keys' rev_done' set_take_auxlist'
+      lookup_a2_map'_keys list_all2'
+    unfolding valid_mmuaux_def add_new_mmuaux_eq valid_mmuaux'.simps I_ivl_w[symmetric] ivl_w'
+      cur_w' b_pos
+    by auto
+qed
+
+lemma list_all2_check_before: "list_all2 (\<lambda>x y. triple_eq_pair x y f g) xs (zip ys zs) \<Longrightarrow>
+  (\<And>y. y \<in> set ys \<Longrightarrow> \<not>enat y + right I < nt) \<Longrightarrow> x \<in> set xs \<Longrightarrow> \<not>check_before I nt x"
+  apply (induction xs "zip ys zs" arbitrary: ys zs rule: list_all2_induct)
+   apply auto
+   apply (metis in_set_zipE list.set_intros(1))
+  by (metis set_subset_Cons subsetD zip_eq_ConsE)
+
+fun eval_mmuaux :: "ts \<Rightarrow> 'a mmuaux \<Rightarrow> 'a table list \<times> 'a mmuaux" where
+  "eval_mmuaux nt aux =
+    (let (tp, len, tss, I, pos, maskL, maskR, a1_map, a2_map, done, done_length) =
+    shift_mmuaux nt aux in
+    (rev done, (tp, len, tss, I, pos, maskL, maskR, a1_map, a2_map, [], 0)))"
+
+lemma valid_eval_mmuaux:
+  assumes "valid_mmuaux w b n L R aux auxlist" "nt \<ge> current w"
+    "eval_mmuaux nt aux = (res, aux')" "eval_until (ivl w) nt auxlist = (res', auxlist')"
+  shows "res = res' \<and> valid_mmuaux w b n L R aux' auxlist'"
+proof -
+  have valid_folded: "valid_mmuaux' w nt b n L R aux auxlist"
+    using assms(1,2) valid_mmuaux'_mono unfolding valid_mmuaux_def by blast
+  obtain tp len tss I pos maskL maskR a1_map a2_map "done" done_length where shift_aux_def:
+    "shift_mmuaux nt aux = (tp, len, tss, I, pos, maskL, maskR, a1_map, a2_map, done, done_length)"
+    by (cases "shift_mmuaux nt aux") auto
+  have valid_shift_aux: "valid_mmuaux' w nt b n L R (tp, len, tss, I, pos, maskL, maskR,
+    a1_map, a2_map, done, done_length) auxlist"
+    "\<And>ts. ts \<in> set (linearize tss) \<Longrightarrow> \<not>enat ts + right (ivl w) < enat nt"
+    using valid_shift_mmuaux'[OF assms(1)[unfolded valid_mmuaux_def] assms(2)]
+    unfolding shift_aux_def by auto
+  have b_pos: "b = pos"
+    using valid_shift_aux unfolding shift_aux_def by auto
+  have I_ivl_w: "I = ivl w"
+    using valid_shift_aux by auto
+  have len_done_auxlist: "length done \<le> length auxlist"
+    using valid_shift_aux by auto
+  have list_all: "\<And>x. x \<in> set (take (length done) auxlist) \<Longrightarrow> check_before I nt x"
+    using valid_shift_aux by auto
+  have set_drop_auxlist: "\<And>x. x \<in> set (drop (length done) auxlist) \<Longrightarrow> \<not>check_before I nt x"
+    using valid_shift_aux[unfolded valid_mmuaux'.simps]
+      list_all2_check_before[OF _ valid_shift_aux(2)] unfolding I_ivl_w by fast
+  have take_auxlist_takeWhile: "take (length done) auxlist = takeWhile (check_before I nt) auxlist"
+    using len_done_auxlist list_all set_drop_auxlist
+    by (rule take_length_takeWhile) assumption+
+  have rev_done: "rev done = map proj_thd (take (length done) auxlist)"
+    using valid_shift_aux by auto
+  then have res'_def: "res' = rev done"
+    using eval_until_res[OF assms(4)] unfolding take_auxlist_takeWhile I_ivl_w by auto
+  then have auxlist'_def: "auxlist' = drop (length done) auxlist"
+    using eval_until_auxlist'[OF assms(4)] by auto
+  have eval_mmuaux_eq: "eval_mmuaux nt aux = (rev done, (tp, len, tss, I, pos, maskL, maskR,
+    a1_map, a2_map, [], 0))"
+    using shift_aux_def by auto
+  show ?thesis
+    using assms(3) done_empty_valid_mmuaux'_intro[OF valid_shift_aux(1)]
+    unfolding shift_aux_def eval_mmuaux_eq b_pos auxlist'_def res'_def valid_mmuaux_def by auto
+qed
+
+definition init_mmuaux :: "\<I> \<Rightarrow> bool \<Rightarrow> nat \<Rightarrow> nat set \<Rightarrow> nat set \<Rightarrow> 'a mmuaux" where
+  "init_mmuaux I pos n L R = (0, 0, empty_queue, I, pos, join_mask n L, join_mask n R,
+    Mapping.empty, Mapping.update 0 Mapping.empty Mapping.empty, [], 0)"
+
+lemma valid_init_mmuaux: "L \<subseteq> R \<Longrightarrow> valid_mmuaux (init_window I) pos n L R
+  (init_mmuaux I pos n L R) []"
+  unfolding init_mmuaux_def valid_mmuaux_def
+  by (auto simp add: init_window_def empty_queue_rep table_def Mapping.lookup_update)
 
 fun length_mmuaux :: "'a mmuaux \<Rightarrow> nat" where
-  "length_mmuaux (t, I, xs) = length xs"
+  "length_mmuaux (tp, len, tss, I, pos, maskL, maskR, a1_map, a2_map, done, done_length) =
+    len + done_length"
 
-fun eval_mmuaux :: "nat \<Rightarrow> 'a mmuaux \<Rightarrow> 'a table list \<times> 'a mmuaux" where
-  "eval_mmuaux nt (t, I, xs) = (let (res, xs') = eval_until I nt xs in (res, (t, I, xs')))"
-
-interpretation default_muaux: muaux valid_mmuaux init_mmuaux add_new_mmuaux length_mmuaux eval_mmuaux
-  by unfold_locales
-    (auto simp add: valid_mmuaux_def init_window_def eval_until_length)
+lemma valid_length_mmuaux:
+  assumes "valid_mmuaux w b n L R aux auxlist"
+  shows "length_mmuaux aux = length auxlist"
+  using assms by (cases aux) (auto simp add: valid_mmuaux_def dest: list_all2_lengthD)
 
 end
